cvc5.lean
@@ -7,13 +7,66 @@ Authors: Abdalrhman Mohamed, Adrien Champion
 
 import Std.Internal.Rat
 
-import cvc5.Init
+import cvc5.NuInit
 import cvc5.Kind
 import cvc5.ProofRule
 import cvc5.SkolemId
 import cvc5.Types
 
-namespace cvc5
+
+
+/-! # Cvc5 low-level API -/
+namespace Cvc5
+
+
+
+/-! ## Basic types -/
+
+
+export cvc5 (
+  Kind SortKind SkolemId
+  ProofRule ProofRewriteRule ProofComponent ProofFormat
+  UnknownExplanation
+  RoundingMode BlockModelsMode
+  LearnedLitType
+  FindSynthTarget InputLanguage
+)
+
+
+
+/-- Error type. -/
+inductive Error where
+  | missingValue
+  | error (msg : String)
+  | recoverable (msg : String)
+  | unsupported (msg : String)
+  | option (msg : String)
+deriving Repr
+
+namespace Error
+
+def toIO : Error → IO.Error
+  | .missingValue => IO.Error.userError "missing value"
+  | .error msg => IO.Error.userError s!"[error] {msg}"
+  | .recoverable msg => IO.Error.userError s!"[recoverable] {msg}"
+  | .unsupported msg => IO.Error.userError s!"[unsupported] {msg}"
+  | .option msg => IO.Error.userError s!"[option] {msg}"
+
+/-- String representation of an error. -/
+protected def toString : Error → String :=
+  toString ∘ repr
+
+/-- Panics on errors, otherwise yields the `ok` result. -/
+def unwrap! [Inhabited α] : Except Error α → α
+| .ok a => a
+| .error e => panic! e.toString
+
+instance : ToString Error :=
+  ⟨Error.toString⟩
+
+end Error
+
+
 
 namespace Kind
 
@@ -228,94 +281,9 @@ private opaque ResultImpl : NonemptyType.{0}
 /-- Encapsulation of a three-valued solver result, with explanations. -/
 def Result : Type := ResultImpl.type
 
-instance Result.instNonemptyResult : Nonempty Result := ResultImpl.property
-
-private opaque SortImpl : NonemptyType.{0}
-
-end cvc5
-
-/-- The sort of a cvc5 term. -/
-def cvc5.Sort : Type := cvc5.SortImpl.type
-
-namespace cvc5
-
-instance Sort.instNonemptySort : Nonempty cvc5.Sort := SortImpl.property
-
-private opaque OpImpl : NonemptyType.{0}
-
-/-- A cvc5 operator.
-
-An operator is a term that represents certain operators, instantiated with its required parameters,
-*e.g.*, a `Term` of kind `Kind.BITVECTOR_EXTRACT`.
--/
-def Op : Type := OpImpl.type
-
-instance Op.instNonemptyOp : Nonempty Op := OpImpl.property
-
-private opaque TermImpl : NonemptyType.{0}
-
-/-- A cvc5 term. -/
-def Term : Type := TermImpl.type
-
-instance Term.instNonemptyTerm : Nonempty Term := TermImpl.property
-
-private opaque ProofImpl : NonemptyType.{0}
-
-/-- A cvc5 proof.
-
-Proofs are trees and every proof object corresponds to the root step of a proof. The branches of the
-root step are the premises of the step.
--/
-def Proof : Type := ProofImpl.type
-
-instance Proof.instNonemptyProof : Nonempty Proof := ProofImpl.property
-
-private opaque TermManagerImpl : NonemptyType.{0}
-
-/-- Manager for cvc5 terms. -/
-def TermManager : Type := TermManagerImpl.type
-
-instance TermManager.instNonemptyTermManager : Nonempty TermManager := TermManagerImpl.property
-
-/-- Error type. -/
-inductive Error where
-  | missingValue
-  | error (msg : String)
-  | recoverable (msg : String)
-  | unsupported (msg : String)
-  | option (msg : String)
-deriving Repr
-
-private opaque SolverImpl : NonemptyType.{0}
-
-/-- A cvc5 solver. -/
-def Solver : Type := SolverImpl.type
-
-instance Solver.instNonemptySolver : Nonempty Solver := SolverImpl.property
-
-/-- Solver error/state-monad transformer. -/
-abbrev SolverT m := ExceptT Error (StateT Solver m)
-
-/-- Solver error/state-monad wrapped in `IO`. -/
-abbrev SolverM := SolverT IO
-
-namespace Error
-
-/-- String representation of an error. -/
-protected def toString : Error → String :=
-  toString ∘ repr
-
-/-- Panics on errors, otherwise yields the `ok` result. -/
-def unwrap! [Inhabited α] : Except Error α → α
-| .ok a => a
-| .error e => panic! e.toString
-
-instance : ToString Error :=
-  ⟨Error.toString⟩
-
-end Error
-
 namespace Result
+
+instance : Nonempty Result := ResultImpl.property
 
 /-- Comparison for structural equality. -/
 protected extern_def beq : Result → Result → Bool
@@ -355,32 +323,61 @@ instance : ToString Result := ⟨Result.toString⟩
 
 end Result
 
+
+
+private opaque ProofImpl : NonemptyType.{0}
+
+/-- A cvc5 proof.
+
+Proofs are trees and every proof object corresponds to the root step of a proof. The branches of the
+root step are the premises of the step.
+-/
+@[irreducible]
+def Proof : (ω : Type) → Type := fun _ => ProofImpl.type
+
+namespace Proof
+
+private theorem typeDef : Proof ω = ProofImpl.type :=
+  by unfold Proof ; rfl
+
+private def toImpl : Proof ω → ProofImpl.type :=
+  by rw [typeDef] ; exact id
+
+private def ofImpl : ProofImpl.type → Proof ω :=
+  by rw [typeDef] ; exact id
+
+instance instNonemptyProof : Nonempty (Proof ω) :=
+  by rw [typeDef] ; exact ProofImpl.property
+
+end Proof
+
+
+
+/-! ## FFI constructor
+
+The following constructors are only used by C++ to inject values as `Except Error _`.
+-/
 section ffi_except_constructors
 
 /-- Only used by FFI to inject values. -/
 @[export except_ok]
-private def mkExceptOk {α : Type} : α → Except Error α :=
-  .ok
+private def mkExceptOk {α : Type} : α → Except Error α := .ok
 
 /-- Only used by FFI to inject values. -/
 @[export except_ok_bool]
-private def mkExceptOkBool : Bool → Except Error Bool :=
-  .ok
+private def mkExceptOkBool : Bool → Except Error Bool := .ok
 
 /-- Only used by FFI to inject values. -/
 @[export except_ok_u32]
-private def mkExceptOkU32 : UInt32 → Except Error UInt32 :=
-  .ok
+private def mkExceptOkU32 : UInt32 → Except Error UInt32 := .ok
 
 /-- Only used by FFI to inject values. -/
 @[export except_ok_u16]
-private def mkExceptOkU16 : UInt16 → Except Error UInt16 :=
-  .ok
+private def mkExceptOkU16 : UInt16 → Except Error UInt16 := .ok
 
 /-- Only used by FFI to inject values. -/
 @[export except_ok_u8]
-private def mkExceptOkU8 : UInt8 → Except Error UInt8 :=
-  .ok
+private def mkExceptOkU8 : UInt8 → Except Error UInt8 := .ok
 
 /-- Only used by FFI to inject errors. -/
 @[export except_err]
@@ -389,151 +386,244 @@ private def mkExceptErr {α : Type} : String → Except Error α :=
 
 end ffi_except_constructors
 
-end cvc5
 
-namespace cvc5.Sort
+
+/-! ## Environment, private `TermManager`, and `Solver`-related definitions -/
+
+
+
+private opaque TermManagerImpl : NonemptyType.{0}
+
+/-- Manager for cvc5 terms. -/
+private def TermManager : Type := TermManagerImpl.type
+
+namespace TermManager
+
+instance : Nonempty TermManager := TermManagerImpl.property
+
+@[extern "termManager_new"]
+private opaque new : Unit → BaseIO TermManager
+
+end TermManager
+
+
+structure Env (ω : Type) (α : Type) where
+private ofRaw ::
+  toRaw : ReaderT Cvc5.TermManager (ExceptT Error BaseIO) α
+
+namespace Env
+
+def run (code : {ω : Type} → Env ω α) : ExceptT Error BaseIO α := do
+  let tm ← TermManager.new ()
+  (@code Unit).toRaw tm
+
+def runIO (code : {ω : Type} → Env ω α) : IO α := fun world =>
+  match run code world with
+  | .ok (.ok res) world => .ok res world
+  | .ok (.error err) world => .error err.toIO world
+
+instance : Monad (Env ω) where
+  pure := (⟨pure ·⟩)
+  bind | ⟨code⟩, f => ⟨fun tm => code tm >>= (f · |>.toRaw tm)⟩
+
+instance : MonadExcept Error (Env ω) where
+  throw e := ⟨fun _ => throw e⟩
+  tryCatch | ⟨code⟩, errorDo => ofRaw fun tm world =>
+    match code tm world with
+    | okay@(.ok (.ok _) _) => okay
+    | error@(.error _ _) => error
+    | .ok (.error e) world => errorDo e |>.toRaw tm world
+
+instance : MonadLift (ST IO.RealWorld) (Env ω) where
+  monadLift stCode := ofRaw fun _ => stCode
+
+instance : MonadLift (Except Error) (Env ω) where
+  monadLift excCode := ofRaw fun _ => excCode
+
+instance : MonadLift IO (Env ω) where
+  monadLift ioCode := ofRaw fun _ => do
+    match ← ioCode.toBaseIO with
+    | .ok res => return res
+    | .error e => throw <| Error.error s!"[IO] {e}"
+
+-- sanity
+example : MonadLiftT BaseIO (Env ω) := inferInstance
+
+private def managerDo (f : TermManager → Env ω α) : Env ω α :=
+  ofRaw fun tm => (f tm |>.toRaw tm)
+
+private def managerDo? (f : TermManager → Except Error α) : Env ω α :=
+  managerDo (liftM ∘ f)
+
+end Env
+
+
+private opaque SrtImpl : NonemptyType.{0}
+
+/-- The sort of a cvc5 term. -/
+@[irreducible]
+def Srt : (ω : Type) → Type := fun _ => SrtImpl.type
+
+namespace Srt
+
+private theorem typeDef : Srt ω = SrtImpl.type :=
+  by unfold Srt ; rfl
+
+private def toImpl : (srt : Srt ω) → SrtImpl.type :=
+  by rw [typeDef] ; exact id
+
+private def ofImpl : (srt : SrtImpl.type) → Srt ω :=
+  by rw [typeDef] ; exact id
+
+instance instNonemptySort : Nonempty (Srt ω) :=
+  by rw [typeDef] ; exact SrtImpl.property
 
 /-- The null sort. -/
-extern_def null : Unit → cvc5.Sort
+private extern_def null : Unit → Srt ω
 
-instance : Inhabited cvc5.Sort := ⟨null ()⟩
+private instance : Inhabited (Srt ω) := ⟨null ()⟩
+
+/-- A string representation of this sort. -/
+protected extern_def toString : Srt ω → String
+
+instance : ToString (Srt ω) := ⟨Srt.toString⟩
 
 /-- Comparison for structural equality. -/
-protected extern_def beq : cvc5.Sort → cvc5.Sort → Bool
+protected extern_def beq : Srt ω → Srt ω → Bool
 
-instance : BEq cvc5.Sort := ⟨Sort.beq⟩
+instance : BEq (Srt ω) := ⟨Srt.beq⟩
 
 /-- Less than comparison. -/
-protected extern_def blt : cvc5.Sort → cvc5.Sort → Bool
+protected extern_def blt : Srt ω → Srt ω → Bool
 
 /-- Greater than comparison. -/
-protected extern_def bgt : cvc5.Sort → cvc5.Sort → Bool
+protected extern_def bgt : Srt ω → Srt ω → Bool
 
 /-- Less than or equal comparison. -/
-protected extern_def ble : cvc5.Sort → cvc5.Sort → Bool
+protected extern_def ble : Srt ω → Srt ω → Bool
 
 /-- Greater than or equal comparison. -/
-protected extern_def bge : cvc5.Sort → cvc5.Sort → Bool
+protected extern_def bge : Srt ω → Srt ω → Bool
 
 /-- Comparison of two sorts. -/
-protected def compare (s1 s2 : cvc5.Sort) : Ordering :=
+protected def compare (s1 s2 : Srt ω) : Ordering :=
   if s1.beq s2 then .eq
   else if s1.bgt s2 then .gt
   else .lt
 
-instance : Ord cvc5.Sort := ⟨Sort.compare⟩
+instance : Ord (Srt ω) := ⟨Srt.compare⟩
 
-instance : LT cvc5.Sort where
-  lt := (Sort.blt · ·)
+instance : LT (Srt ω) where
+  lt := (Srt.blt · ·)
 
-instance : DecidableLT cvc5.Sort :=
+instance : DecidableLT (Srt ω) :=
   fun s1 s2 => if h : s1.blt s2 then .isTrue h else .isFalse h
 
-instance : LE cvc5.Sort where
-  le := (Sort.ble · ·)
+instance : LE (Srt ω) where
+  le := (Srt.ble · ·)
 
-instance : DecidableLE cvc5.Sort :=
+instance : DecidableLE (Srt ω) :=
   fun s1 s2 => if h : s1.ble s2 then .isTrue h else .isFalse h
 
 /-- Hash function for cvc5 sorts. -/
-protected extern_def hash : cvc5.Sort → UInt64
+protected extern_def hash : Srt ω → UInt64
 
-instance : Hashable cvc5.Sort := ⟨Sort.hash⟩
+instance : Hashable (Srt ω) := ⟨Srt.hash⟩
 
 /-- Get the kind of this sort. -/
-extern_def getKind : cvc5.Sort → SortKind
+extern_def getKind : Srt ω → SortKind
 
-/-- Determine if this is the null sort (`cvc5.Sort`). -/
-extern_def isNull : cvc5.Sort → Bool
+/-- Determine if this is the null sort. -/
+extern_def isNull : Srt ω → Bool
 
 /-- Determine if this is the Boolean sort (SMT-LIB: `Bool`). -/
-extern_def isBoolean : cvc5.Sort → Bool
+extern_def isBoolean : Srt ω → Bool
 
 /-- Determine if this is the Integer sort (SMT-LIB: `Int`). -/
-extern_def isInteger : cvc5.Sort → Bool
+extern_def isInteger : Srt ω → Bool
 
 /-- Determine if this is the Real sort (SMT-LIB: `Real`). -/
-extern_def isReal : cvc5.Sort → Bool
+extern_def isReal : Srt ω → Bool
 
 /-- Determine if this is the String sort (SMT-LIB: `String`). -/
-extern_def isString : cvc5.Sort → Bool
+extern_def isString : Srt ω → Bool
 
 /-- Determine if this is the regular expression sort (SMT-LIB: `RegLan`). -/
-extern_def isRegExp : cvc5.Sort → Bool
+extern_def isRegExp : Srt ω → Bool
 
 /-- Determine if this is the rounding mode sort (SMT-LIB: `RoundingMode`). -/
-extern_def isRoundingMode : cvc5.Sort → Bool
+extern_def isRoundingMode : Srt ω → Bool
 
 /-- Determine if this is a bit-vector sort (SMT-LIB: `(_ BitVec i)`). -/
-extern_def isBitVector : cvc5.Sort → Bool
+extern_def isBitVector : Srt ω → Bool
 
 /-- Determine if this is a floating-point sort (SMT-LIB: `(_ FloatingPoint eb sb)`). -/
-extern_def isFloatingPoint : cvc5.Sort → Bool
+extern_def isFloatingPoint : Srt ω → Bool
 
 /-- Determine if this is a datatype sort. -/
-extern_def isDatatype : cvc5.Sort → Bool
+extern_def isDatatype : Srt ω → Bool
 
 /-- Determine if this is a datatype constructor sort. -/
-extern_def isDatatypeConstructor : cvc5.Sort → Bool
+extern_def isDatatypeConstructor : Srt ω → Bool
 
 /-- Determine if this is a datatype selector sort. -/
-extern_def isDatatypeSelector : cvc5.Sort → Bool
+extern_def isDatatypeSelector : Srt ω → Bool
 
 /-- Determine if this is a datatype tester sort. -/
-extern_def isDatatypeTester : cvc5.Sort → Bool
+extern_def isDatatypeTester : Srt ω → Bool
 
 /-- Determine if this is a datatype updater sort. -/
-extern_def isDatatypeUpdater : cvc5.Sort → Bool
+extern_def isDatatypeUpdater : Srt ω → Bool
 
 /-- Determine if this is a function sort. -/
-extern_def isFunction : cvc5.Sort → Bool
+extern_def isFunction : Srt ω → Bool
 
 /-- Determine if this is a predicate sort.
 
 A predicate sort is a function sort that maps to the Boolean sort. All predicate sorts are also
 function sorts.
 -/
-extern_def isPredicate : cvc5.Sort → Bool
+extern_def isPredicate : Srt ω → Bool
 
 /-- Determine if this is a tuple sort. -/
-extern_def isTuple : cvc5.Sort → Bool
+extern_def isTuple : Srt ω → Bool
 
 /-- Determine if this is a nullable sort. -/
-extern_def isNullable : cvc5.Sort → Bool
+extern_def isNullable : Srt ω → Bool
 
 /-- Determine if this is a record sort.
 
 **Warning**: this function is experimental and may change in future versions.
 -/
-extern_def isRecord : cvc5.Sort → Bool
+extern_def isRecord : Srt ω → Bool
 
 /-- Determine if this is an array sort. -/
-extern_def isArray : cvc5.Sort → Bool
+extern_def isArray : Srt ω → Bool
 
 /-- Determine if this is a finite field sort. -/
-extern_def isFiniteField : cvc5.Sort → Bool
+extern_def isFiniteField : Srt ω → Bool
 
 /-- Determine if this is a Set sort. -/
-extern_def isSet : cvc5.Sort → Bool
+extern_def isSet : Srt ω → Bool
 
 /-- Determine if this is a Bag sort. -/
-extern_def isBag : cvc5.Sort → Bool
+extern_def isBag : Srt ω → Bool
 
 /-- Determine if this is a Sequence sort. -/
-extern_def isSequence : cvc5.Sort → Bool
+extern_def isSequence : Srt ω → Bool
 
 /-- Determine if this is an abstract sort. -/
-extern_def isAbstract : cvc5.Sort → Bool
+extern_def isAbstract : Srt ω → Bool
 
 /-- Determine if this is an uninterpreted sort. -/
-extern_def isUninterpretedSort : cvc5.Sort → Bool
+extern_def isUninterpretedSort : Srt ω → Bool
 
 /-- Determine if this is an uninterpreted sort constructor.
 
 An uninterpreted sort constructor has arity `> 0` and can be instantiated to construct uninterpreted
 sorts with given sort parameters.
 -/
-extern_def isUninterpretedSortConstructor : cvc5.Sort → Bool
+extern_def isUninterpretedSortConstructor : Srt ω → Bool
 
 /-- Determine if this is an instantiated (parametric datatype or uninterpreted sort constructor)
 sort.
@@ -541,80 +631,77 @@ sort.
 An instantiated sort is a sort that has been constructed from instantiating a sort with sort
 arguments --- see also `cvc5.Sort.instantiate`.
 -/
-extern_def isInstantiated : cvc5.Sort → Bool
-
-/-- A string representation of this sort. -/
-protected extern_def toString : cvc5.Sort → String
+extern_def isInstantiated : Srt ω → Bool
 
 /-- Determine if this term has a symbol (a name).
 
 For example, free constants and variables have symbols.
 -/
-extern_def!? hasSymbol : cvc5.Sort → Except Error Bool
+extern_def!? hasSymbol : Srt ω → Except Error Bool
 
 /-- Get the symbol of this sort.
 
-The symbol of this sort is the string that was provided when consrtucting it *via* one of
+The symbol of this sort is the string that was provided when constructing it *via* one of
 `Solver.mkUninterpretedSort`, `Solver.mkUnresolvedSort`, or
 `Solver.mkUninterpretedSortConstructorSort`.
 -/
-extern_def!? getSymbol : cvc5.Sort → Except Error String
+extern_def!? getSymbol : Srt ω → Except Error String
 
 /-- The arity of a function sort. -/
-extern_def!? getFunctionArity : cvc5.Sort → Except Error Nat
+extern_def!? getFunctionArity : Srt ω → Except Error Nat
 
 /-- The domain sorts of a function sort. -/
-extern_def!? getFunctionDomainSorts : cvc5.Sort → Except Error (Array cvc5.Sort)
+extern_def!? getFunctionDomainSorts : Srt ω → Except Error (Array (Srt ω))
 
 /-- The codomain sort of a function sort. -/
-extern_def!? getFunctionCodomainSort : cvc5.Sort → Except Error cvc5.Sort
+extern_def!? getFunctionCodomainSort : Srt ω → Except Error (Srt ω)
 
 /-- The array index sort of an array index. -/
-extern_def!? getArrayIndexSort : cvc5.Sort → Except Error cvc5.Sort
+extern_def!? getArrayIndexSort : Srt ω → Except Error (Srt ω)
 
 /-- The array element sort of an array index. -/
-extern_def!? getArrayElementSort : cvc5.Sort → Except Error cvc5.Sort
+extern_def!? getArrayElementSort : Srt ω → Except Error (Srt ω)
 
 /-- The element sort of a set sort. -/
-extern_def!? getSetElementSort : cvc5.Sort → Except Error cvc5.Sort
+extern_def!? getSetElementSort : Srt ω → Except Error (Srt ω)
 
 /-- The element sort of a bag sort. -/
-extern_def!? getBagElementSort : cvc5.Sort → Except Error cvc5.Sort
+extern_def!? getBagElementSort : Srt ω → Except Error (Srt ω)
 
 /-- The element sort of a sequence sort. -/
-extern_def!? getSequenceElementSort : cvc5.Sort → Except Error cvc5.Sort
+extern_def!? getSequenceElementSort : Srt ω → Except Error (Srt ω)
 
 /-- The sort kind of an abstract sort, which denotes the kind of sorts that this abstract sort
 denotes.
 -/
-extern_def!? getAbstractedKind : cvc5.Sort → Except Error SortKind
+extern_def!? getAbstractedKind : Srt ω → Except Error SortKind
 
 /-- The arity of an uninterpreted sort constructor sort. -/
-extern_def!? getUninterpretedSortConstructorArity : cvc5.Sort → Except Error UInt32
+extern_def!? getUninterpretedSortConstructorArity : Srt ω → Except Error UInt32
 
 /-- The bit-width of the bit-vector sort. -/
-extern_def!? getBitVectorSize : cvc5.Sort → Except Error UInt32
+extern_def!? getBitVectorSize : Srt ω → Except Error UInt32
 
 /-- The size of the finite field sort. -/
-extern_def!? getFiniteFieldSize : cvc5.Sort → Except Error Nat
+extern_def!? getFiniteFieldSize : Srt ω → Except Error Nat
 
 /-- The bit-width of the exponent of the floating-point sort. -/
-extern_def!? getFloatingPointExponentSize : cvc5.Sort → Except Error UInt32
+extern_def!? getFloatingPointExponentSize : Srt ω → Except Error UInt32
 
 /-- The width of the significand of the floating-point sort. -/
-extern_def!? getFloatingPointSignificandSize : cvc5.Sort → Except Error UInt32
+extern_def!? getFloatingPointSignificandSize : Srt ω → Except Error UInt32
 
 /-- The length of a tuple sort. -/
-extern_def!? getTupleLength : cvc5.Sort → Except Error UInt32
+extern_def!? getTupleLength : Srt ω → Except Error UInt32
 
 /-- The element sorts of a tuple sort. -/
-extern_def!? getTupleSorts : cvc5.Sort → Except Error (Array cvc5.Sort)
+extern_def!? getTupleSorts : Srt ω → Except Error (Array (Srt ω))
 
 /-- The element sort of a nullable sort. -/
-extern_def!? getNullableElementSort : cvc5.Sort → Except Error cvc5.Sort
+extern_def!? getNullableElementSort : Srt ω → Except Error (Srt ω)
 
 /-- Get the associated uninterpreted sort constructor of an instantiated uninterpreted sort. -/
-extern_def!? getUninterpretedSortConstructor : cvc5.Sort → Except Error cvc5.Sort
+extern_def!? getUninterpretedSortConstructor : Srt ω → Except Error (Srt ω)
 
 /-- Instantiate a parameterized datatype sort or uninterpreted sort constructor sort.
 
@@ -622,537 +709,65 @@ Create sort parameters with `TermManager.mkParamSort symbol`.
 
 - `params` The list of sort parameters to instantiate with.
 -/
-extern_def!? instantiate : cvc5.Sort → (params : Array cvc5.Sort) → Except Error cvc5.Sort
+extern_def!? instantiate : Srt ω → (params : Array (Srt ω)) → Except Error (Srt ω)
 
-/-- Simultaneous substitution of Sorts.
+end Srt
 
-Note that this replacement is applied during a pre-order traversal and only once to the sort. It is not run until fix point. In the case that `sorts` contains duplicates, the replacement earliest in
-the vector takes priority.
 
-**Warning:** This function is experimental and may change in future versions.
 
-- `sorts` The sub-sorts to be substituted within this sort.
-- `replacements` The sort replacing the substituted sub-sorts.
--/
-extern_def!? substitute
-: cvc5.Sort → (sorts : Array cvc5.Sort) → (replacements : Array cvc5.Sort) → Except Error cvc5.Sort
+private opaque TermImpl : NonemptyType.{0}
 
-instance : ToString cvc5.Sort := ⟨Sort.toString⟩
-instance : Repr cvc5.Sort := ⟨fun self _ => self.toString⟩
-
-end cvc5.Sort
-
-namespace cvc5.Op
-
-/-- The null operator. -/
-extern_def null : Unit → Op
-
-instance : Inhabited Op := ⟨null ()⟩
-
-/-- Syntactic equality operator. -/
-protected extern_def beq : Op → Op → Bool
-
-instance : BEq Op := ⟨Op.beq⟩
-
-/-- Get the kind of this operator. -/
-extern_def getKind : Op → Kind
-
-/-- Determine if this operator is nullary. -/
-extern_def isNull : Op → Bool
-
-/-- Determine if this operator is indexed. -/
-extern_def isIndexed : Op → Bool
-
-/-- Get the number of indices of this operator. -/
-extern_def getNumIndices : Op → Nat
-
-/-- Get the index at position `i` of an indexed operator. -/
-protected extern_def get : (op : Op) → Fin op.getNumIndices → Term
-
-/-- Get the string representation of this operator. -/
-protected extern_def toString : Op → String
-
-instance : GetElem Op Nat Term fun op i => i < op.getNumIndices where
-  getElem op i h := op.get ⟨i, h⟩
-
-instance : ToString Op := ⟨Op.toString⟩
-
-end Op
+/-- A cvc5 term. -/
+@[irreducible]
+def Term : (ω : Type) → Type := fun _ => TermImpl.type
 
 namespace Term
 
-/-- The null term. -/
-extern_def null : Unit → Term
+private theorem typeDef : Term ω = TermImpl.type :=
+  by unfold Term ; rfl
 
-instance : Inhabited Term := ⟨null ()⟩
+private def toImpl : Term ω → TermImpl.type :=
+  by rw [typeDef] ; exact id
 
-/-- Syntactic equality operator. -/
-protected extern_def beq : Term → Term → Bool
+private def ofImpl : TermImpl.type → Term ω :=
+  by rw [typeDef] ; exact id
 
-instance : BEq Term := ⟨Term.beq⟩
+instance instNonemptyTerm : Nonempty (Term ω) :=
+  by rw [typeDef] ; exact TermImpl.property
 
-protected extern_def hash : Term → UInt64
+@[extern "term_null"]
+private opaque null : Unit → Term ω
 
-instance : Hashable Term := ⟨Term.hash⟩
-
-/-- Determine if this term is nullary. -/
-extern_def isNull : Term → Bool
-
-/-- Get the kind of this term. -/
-extern_def getKind : Term → Kind
-
-/-- Get the sort of this term. -/
-extern_def getSort : Term → cvc5.Sort
-
-/-- Determine if this term has an operator. -/
-extern_def hasOp : Term → Bool
-
-/-- Determine if this term has a symbol (a name).
-
-For example, free constants and variables have symbols.
--/
-extern_def hasSymbol : Term → Bool
-
-/-- Get the id of this term. -/
-extern_def getId : Term → Nat
-
-/-- Get the number of children of this term. -/
-extern_def getNumChildren : Term → Nat
-
-/-- Is this term a skolem? -/
-extern_def isSkolem : Term → Bool
-
-/-- Get the child term of this term at a given index. -/
-protected extern_def get : (t : Term) → Fin t.getNumChildren → Term
-
-/-- Get the operator of a term with an operator.
-
-Requires that this term has an operator (see `hasOp`).
--/
-extern_def!? getOp : Term → Except Error Op
-
-/-- Get the value of a Boolean term as a native Boolean value.
-
-Requires `term` to have sort Bool.
--/
-extern_def!? getBooleanValue : Term → Except Error Bool
-
-/-- Get the string representation of a bit-vector value.
-
-Requires `term` to have a bit-vector sort.
-
-- `base`: `2` for binary, `10` for decimal, and `16` for hexadecimal.
--/
-extern_def!? getBitVectorValue : Term → UInt32 → Except Error String
-
-/-- Get the native integral value of an integral value. -/
-extern_def!? getIntegerValue : Term → Except Error Int
-
-/-- Get the native rational value of a real, rational-compatible value. -/
-extern_def!? getRationalValue : Term → Except Error Std.Internal.Rat
-
-/-- Get the symbol of this term.
-
-Requires that this term has a symbol (see `hasSymbol`).
-
-The symbol of the term is the string that was provided when constructing it *via*
-`TermManager.mkConst` or `TermManager.mkVar`.
--/
-extern_def!? getSymbol : Term → Except Error String
-
-/-- Get skolem identifier of this term.
-
-Requires `isSkolem`.
--/
-extern_def!? getSkolemId : Term → Except Error SkolemId
-
-/-- Get the skolem indices of this term.
-
-Requires `isSkolem`.
-
-Returns the skolem indices of this term. This is a list of terms that the skolem function is indexed
-by. For example, the array diff skolem `SkolemId.ARRAY_DEQ_DIFF` is indexed by two arrays.
--/
-extern_def!? getSkolemIndices : Term → Except Error (Array Term)
-
-instance : GetElem Term Nat Term fun t i => i < t.getNumChildren where
-  getElem t i h := t.get ⟨i, h⟩
-
-protected def forIn {β : Type u} [Monad m] (t : Term) (b : β) (f : Term → β → m (ForInStep β)) : m β :=
-  let rec loop (i : Nat) (h : i ≤ t.getNumChildren) (b : β) : m β := do
-    match i, h with
-    | 0,   _ => pure b
-    | i+1, h =>
-      have h' : i < t.getNumChildren := Nat.lt_of_lt_of_le (Nat.lt_succ_self i) h
-      have : t.getNumChildren - 1 < t.getNumChildren := Nat.sub_lt (Nat.zero_lt_of_lt h') (by decide)
-      have : t.getNumChildren - 1 - i < t.getNumChildren := Nat.lt_of_le_of_lt (Nat.sub_le (t.getNumChildren - 1) i) this
-      match (← f t[t.getNumChildren - 1 - i] b) with
-      | ForInStep.done b  => pure b
-      | ForInStep.yield b => loop i (Nat.le_of_lt h') b
-  loop t.getNumChildren (Nat.le_refl _) b
-
-instance : ForIn m Term Term where
-  forIn := Term.forIn
-
-/-- Get the children of a term. -/
-def getChildren (t : Term) : Array Term := Id.run do
-  let mut cts := #[]
-  for ct in t do
-    cts := cts.push ct
-  cts
-
-/-- Boolean negation. -/
-protected extern_def!? not : (t : Term) → Except Error Term
-
-/-- Boolean and. -/
-protected extern_def!? and : (lft rgt : Term) → Except Error Term
-
-/-- Boolean or. -/
-protected extern_def!? or : (lft rgt : Term) → Except Error Term
-
-/-- Boolean exclusive or. -/
-protected extern_def!? xor : (lft rgt : Term) → Except Error Term
-
-/-- Equality. -/
-protected extern_def!? eq : (lft rgt : Term) → Except Error Term
-
-/-- Boolean implication. -/
-protected extern_def!? imp : (lft rgt : Term) → Except Error Term
-
-/-- If-then-else.
-
-- `cnd`: condition, must be a Boolean term;
-- `thn`: then-branch of some sort `S`;
-- `els`: else-branch of *the same* sort `S`.
--/
-protected extern_def!? ite : (cnd thn els : Term) → Except Error Term
+instance : Inhabited (Term ω) := ⟨null ()⟩
 
 /-- A string representation of this term. -/
-protected extern_def toString : Term → String
+protected extern_def toString : Term ω → String
 
-instance : ToString Term := ⟨Term.toString⟩
+instance : ToString (Term ω) := ⟨Term.toString⟩
 
 end Term
 
-namespace Proof
 
-/-- The null proof. -/
-extern_def null : Unit → Proof
 
-instance : Inhabited Proof := ⟨null ()⟩
+private opaque SolverImpl : NonemptyType.{0}
 
-/-- Get the proof rule used by the root step of the root. -/
-extern_def getRule : Proof → ProofRule
+/-- A cvc5 solver. -/
+private def Solver.Raw : Type := SolverImpl.type
 
-/-- Get the proof rewrite rule used by the root step of the proof.
+namespace Solver.Raw
 
-Requires that `getRule` does not return `ProofRule.DSL_REWRITE` or `ProofRule.REWRITE`.
--/
-extern_def!? getRewriteRule : Proof → Except Error ProofRewriteRule
+instance : Nonempty Solver.Raw := SolverImpl.property
 
-/-- The conclusion of the root step of the proof. -/
-extern_def getResult : Proof → Term
+end Solver.Raw
 
-/-- The premises of the root step of the proof. -/
-extern_def getChildren : Proof → Array Proof
-
-/-- The arguments of the root step of the proof as a vector of terms.
-
-Some of those terms might be strings.
--/
-extern_def getArguments : Proof → Array Term
-
-/-- Operator overloading for referential equality of two proofs. -/
-protected extern_def beq : Proof → Proof → Bool
-
-instance : BEq Proof := ⟨Proof.beq⟩
-
-/-- Hash function for proofs. -/
-protected extern_def hash : Proof → UInt64
-
-instance : Hashable Proof := ⟨Proof.hash⟩
-
-end Proof
-
-namespace TermManager
-
-/-- Constructor. -/
-extern_def new : BaseIO TermManager
-
-/-- Get the Boolean sort. -/
-extern_def getBooleanSort : TermManager → cvc5.Sort
-
-/-- Get the Integer sort. -/
-extern_def getIntegerSort : TermManager → cvc5.Sort
-
-/-- Get the Real sort. -/
-extern_def getRealSort : TermManager → cvc5.Sort
-
-/-- Get the regular expression sort. -/
-extern_def getRegExpSort : TermManager → cvc5.Sort
-
-/-- Get the rounding mode sort. -/
-extern_def getRoundingModeSort : TermManager → cvc5.Sort
-
-/-- Get the string sort. -/
-extern_def getStringSort : TermManager → cvc5.Sort
-
-/-- Create an array sort.
-
-- `indexSort` The array index sort.
-- `elemSort` The array element sort.
--/
-extern_def!? mkArraySort : TermManager → (indexSort elemSort : cvc5.Sort) → Except Error cvc5.Sort
-
-/-- Create a bit-vector sort.
-
-- `size` The bit-width of the bit-vector sort.
--/
-extern_def!? mkBitVectorSort : TermManager → (size : UInt32) → Except Error cvc5.Sort
-
-/-- Create a floating-point sort.
-
-- `exp` The bit-width of the exponent of the floating-point sort.
-- `sig` The bit-width of the significand of the floating-point sort.
--/
-extern_def!? mkFloatingPointSort : TermManager → (exp sig : UInt32) → Except Error cvc5.Sort
-
-/-- Create a finite-field sort from a given string of base n.
-
-- `size` The modulus of the field. Must be a prime.
--/
-private extern_def mkFiniteFieldSortFromString : TermManager → (size : String) → (base : UInt32 := 10) → Except Error cvc5.Sort
-
-@[inherit_doc mkFiniteFieldSortFromString]
-abbrev mkFiniteFieldSort (tm : TermManager) : (size : Nat) → Except Error cvc5.Sort :=
-  (tm.mkFiniteFieldSortFromString · 10) ∘ toString
-@[inherit_doc mkFiniteFieldSortFromString]
-abbrev mkFiniteFieldSort! (tm : TermManager) : (size : Nat) → cvc5.Sort :=
-  Error.unwrap! ∘ (tm.mkFiniteFieldSortFromString · 10) ∘ toString
-@[inherit_doc mkFiniteFieldSortFromString]
-abbrev mkFiniteFieldSort? (tm : TermManager) : (size : Nat) → Option cvc5.Sort :=
-  Except.toOption ∘ (tm.mkFiniteFieldSortFromString · 10) ∘ toString
-
-/-- Create function sort.
-
-- `sorts` The sort of the function arguments.
-- `codomain` The sort of the function return value.
--/
-extern_def!? mkFunctionSort
-: TermManager → (sorts : Array cvc5.Sort) → (codomain : cvc5.Sort) → Except Error cvc5.Sort
-
-/-- Create a predicate sort.
-
-This is equivalent to calling `mkFunctionSort` with Boolean sort as the codomain.
-
-- `sorts` The list of sorts of the predicate.
--/
-extern_def!? mkPredicateSort : TermManager → (sorts : Array cvc5.Sort) → Except Error cvc5.Sort
-
-/-- Create a tuple sort.
-
-- `sorts` The sorts of the elements of the tuple.
--/
-extern_def!? mkTupleSort : TermManager → (sorts : Array cvc5.Sort) → Except Error cvc5.Sort
-
-/-- Create an uninterpreted sort constructor sort.
-
-An uninterpreted sort constructor is an uninterpreted sort with arity > 0.
-
-- `arity` The arity of the sort (must be > 0).
-- `symbol` The symbol of the sort.
--/
-extern_def!? mkUninterpretedSortConstructorSort
-: TermManager → (arity : Nat) → (symbol : String) → Except Error cvc5.Sort
-
-/-- Create a set parameter.
-
-- `elemSort` The sort of the set elements.
--/
-extern_def!? mkSetSort : TermManager → (sort : cvc5.Sort) → Except Error cvc5.Sort
-
-/-- Create a set parameter.
-
-- `elemSort` The sort of the set elements.
--/
-extern_def!? mkBagSort : TermManager → (sort : cvc5.Sort) → Except Error cvc5.Sort
-
-/-- Create a set parameter.
-
-- `elemSort` The sort of the set elements.
--/
-extern_def!? mkSequenceSort : TermManager → (sort : cvc5.Sort) → Except Error cvc5.Sort
-
-/-- Create an abstract sort. An abstract sort represents a sort for a given kind whose parameters
-and arguments are unspecified.
-
-The kind `k` must be the kind of a sort that can be abstracted, *i.e.* a sort that has indices or
-arguments sorts. For example, `SortKind.ARRAY_SORT` and `SortKind.BITVECTOR_SORT` can be passed as
-the kind `k` to this function, while `SortKind.INTEGER_SORT` and `SortKind.STRING_SORT` cannot.
-
-**NB:** Providing the kind `SortKind.ABSTRACT_SORT` as an argument to this function returns the
-(fully) unspecified sort, denoted `?`.
-
-**NB:** Providing a kind `k` that has no indices and a fixed arity of argument sorts will return the
-sort of kind `k` whose arguments are the unspecified sort. For example, `mkAbstractSort
-SortKind.ARRAY_SORT` will return the sort `(ARRAY_SORT ? ?)` instead of the abstract sort whose
-abstract kind is `SortKind.ARRAY_SORT`.
--/
-extern_def!? mkAbstractSort : TermManager → (k : SortKind) → Except Error cvc5.Sort
-
-/-- Create an uninterpreted sort.
-
-- `symbol` The name of the sort.
--/
-extern_def mkUninterpretedSort : TermManager → (symbol : String) → cvc5.Sort
-
-/-- Create a nullable sort.
-
-- `sort` The sort of the element of the nullable.
--/
-extern_def!? mkNullableSort : TermManager → (sort : cvc5.Sort) → Except Error cvc5.Sort
-
-/-- Create a sort parameter.
-
-- `symbol` The name of the sort.
-
-**Warning**: This function is experimental and may change in future versions.
--/
-extern_def mkParamSort : TermManager → (symbol : String) → cvc5.Sort
-
-/-- Create a Boolean constant.
-
-- `b`: The Boolean constant.
--/
-extern_def mkBoolean : TermManager → (b : Bool) → Term
-
-/-- Create an integer-value term.
-
-- `s`: the string representation of the constant, may represent an integer such as (`"123"`).
--/
-private extern_def mkIntegerFromString : TermManager → (s : String) → Except Error Term
-with
-  /-- Create an integer-value term. -/
-  mkInteger (tm : TermManager) : Int → Term :=
-    Error.unwrap! ∘ tm.mkIntegerFromString ∘ toString
-
-/-- Create a real-value term.
-
-- `s`: the string representation of the constant, may represent an integer (`"123"`) or a real
-  constant (`"12.34"`, `"12/34"`).
--/
-private extern_def mkRealFromString : TermManager → (s : String) → Except Error Term
-with
-  /-- Create a real-value term from a `Std.Internal.Rat`. -/
-  mkRealOfRat (tm : TermManager) (rat : Std.Internal.Rat) : Term :=
-    tm.mkRealFromString s!"{rat.num}/{rat.den}" |> Error.unwrap!
-  /-- Create a real-value term from numerator/denominator `Int`-s. -/
-  mkReal (tm : TermManager)
-    (num : Int) (den : Int := 1) (den_ne_0 : den ≠ 0 := by simp <;> omega)
-  : Term :=
-    let (num, den) :=
-      match h : den with
-      | .ofNat 0 => by contradiction
-      | .ofNat den => (num, den)
-      | .negSucc denMinus1 => (-num, denMinus1.succ)
-    tm.mkRealOfRat <| Std.Internal.mkRat num den
-
-/-- Create operator of Kind:
-
-- `Kind.BITVECTOR_EXTRACT`
-- `Kind.BITVECTOR_REPEAT`
-- `Kind.BITVECTOR_ROTATE_LEFT`
-- `Kind.BITVECTOR_ROTATE_RIGHT`
-- `Kind.BITVECTOR_SIGN_EXTEND`
-- `Kind.BITVECTOR_ZERO_EXTEND`
-- `Kind.DIVISIBLE`
-- `Kind.FLOATINGPOINT_TO_FP_FROM_FP`
-- `Kind.FLOATINGPOINT_TO_FP_FROM_IEEE_BV`
-- `Kind.FLOATINGPOINT_TO_FP_FROM_REAL`
-- `Kind.FLOATINGPOINT_TO_FP_FROM_SBV`
-- `Kind.FLOATINGPOINT_TO_FP_FROM_UBV`
-- `Kind.FLOATINGPOINT_TO_SBV`
-- `Kind.FLOATINGPOINT_TO_UBV`
-- `Kind.INT_TO_BITVECTOR`
-- `Kind.TUPLE_PROJECT`
-
-See `cvc5.Kind` for a description of the parameters.
-
-- `kind` The kind of the operator.
-- `args` The arguments (indices) of the operator.
-
-If `args` is empty, the `Op` simply wraps the `cvc5.Kind`. The `Kind` can be used in
-`Solver.mkTerm` directly without creating an `Op` first.
--/
-extern_def!? mkOpOfIndices : TermManager → (kind : Kind) → (args : Array Nat := #[]) → Except Error Op
-
-@[inherit_doc mkOpOfIndices]
-abbrev mkOp := @mkOpOfIndices
-@[inherit_doc mkOpOfIndices!]
-abbrev mkOp! := @mkOpOfIndices!
-@[inherit_doc mkOpOfIndices?]
-abbrev mkOp? := @mkOpOfIndices?
-
-/-- Create operator of kind:
-
-- `Kind.DIVISIBLE` (to support arbitrary precision integers)
-
-See `cvc5.Kind` for a description of the parameters.
-
-- `kind` The kind of the operator.
-- `arg` The string argument to this operator.
--/
-extern_def!? mkOpOfString : TermManager → (kind : Kind) → (arg : String) → Except Error Op
-
-/-- Create n-ary term of given kind.
-
-- `kind` The kind of the term.
-- `children` The children of the term.
--/
-extern_def!? mkTerm : TermManager → (kind : Kind) → (children : Array Term := #[]) → Except Error Term
-
-/-- Create n-ary term of given kind from a given operator.
-
-Create operators with `mkOp`.
-
-- `op` The operator.
-- `children` The children of the term.
--/
-extern_def!? mkTermOfOp : TermManager → (op : Op) → (children : Array Term := #[]) → Except Error Term
-
-/-- **THIS FUNCTION MUST NOT BE EXPOSED.**
-
-**It produces a different (fresh) term every time it's called which is really bad for purity.**
-
-Create a free constant.
-
-Note that the returned term is always fresh, even if the same arguments were provided on a
-previous call to `mkConst`.
-
-- `sort` The sort of the constant.
-- `symbol` The name of the constant (optional).
--/
-private
-def mkConst (_ : TermManager) (_ : cvc5.Sort) (_ : String := "") : Term :=
-  panic! "illegal call to `cvc5.TermManager.mkConst"
-
-end TermManager
+structure Solver (ω : Type) where
+private mk' ::
+  /-- Underlying raw solver. -/
+  private toRaw : Solver.Raw
+  /-- Parser placeholder. -/
+  private parser : IO.Ref (Option Unit)
 
 namespace Solver
-
-variable [Monad m]
-
-/-- Only used by FFI to wrap *success* results. -/
-@[export solver_val]
-private def val (a : α) : SolverT m α := pure a
-
-/-- Only used by FFI to wrap errors. -/
-@[export solver_err]
-private def err (e : Error) : SolverT m α := throw e
-
-/-- Only used by FFI to wrap cvc5 errors. -/
-@[export solver_errOfString]
-private def errorOfString (msg : String) : SolverT m α := throw (.error msg)
 
 /-- Constructor.
 
@@ -1160,136 +775,979 @@ Constructs solver instance from a given term manager instance.
 
 - `tm`: The associated term manager.
 -/
-private extern_def new : TermManager → Solver
+@[extern "solver_new"]
+private opaque Raw.new : TermManager → Solver.Raw
 
-/-- Get a string representation of the version of this solver. -/
-extern_def getVersion : SolverT m String
+private def ofManager (tm : TermManager) : BaseIO (Solver ω) := do
+  let parser ← IO.mkRef none
+  return {toRaw := Raw.new tm, parser}
 
-/-- Set option.
+def new : Env ω (Solver ω) := Env.managerDo (liftM ∘ ofManager)
 
-- `option`: The option name.
-- `value`: The option value.
--/
-extern_def setOption (option value : String) : SolverT m Unit
+section variable (solver : Solver ω)
 
-/-- Remove all assertions. -/
-extern_def resetAssertions : SolverT m Unit
+private def rawSolverDo (f : Solver.Raw → Env ω α) : Env ω α :=
+  f solver.toRaw
 
-/-- Set logic.
+private def rawSolverDo? (f : Solver.Raw → Except Error α) : Env ω α :=
+  solver.rawSolverDo (liftM ∘ f)
 
-- `logic`: The logic to set.
--/
-extern_def setLogic : (logic : String) → SolverT m Unit
+@[extern "Solver_declareFun"]
+private opaque Raw.declareFun : (solver : Raw)
+→ (symbol : String) → (sorts : Array (Srt ω)) → (sort : Srt ω) → (fresh : Bool)
+→ Except Error (Term ω)
 
-/-- Simplify a term or formula based on rewriting and (optionally) applying substitutions for
-solved variables.
+def declareFun (symbol : String)
+  (sorts : Array (Srt ω)) (sort : Srt ω) (fresh : Bool := false)
+: Env ω (Term ω) :=
+  solver.toRaw.declareFun symbol sorts sort fresh
 
-If `applySubs` is true, then for example, if `(= x 0)` was asserted to this solver, this function
-may replace occurrences of `x` with `0`.
-
-- `t` The term to simplify.
-- `applySubs` True to apply substitutions for solved variables.
--/
-extern_def simplify : (term : Term) → (applySubs : Bool := false) → SolverT m Term
-
-/--
-Declare n-ary function symbol.
-
-SMT-LIB:
-
-\verbatim embed:rst:leading-asterisk
- .. code:: smtlib
-
-     (declare-fun <symbol> ( <sort>* ) <sort>)
- \endverbatim
-
-- `symbol`: The name of the function.
-- `sorts`: The sorts of the parameters to this function.
-- `sort`: The sort of the return value of this function.
-- `fresh`: If true, then this method always returns a new Term. Otherwise, this method will always
-  return the same Term for each call with the given sorts and symbol where fresh is false.
--/
-extern_def declareFun (symbol : String) (sorts : Array cvc5.Sort) (sort : cvc5.Sort) (fresh := true) : SolverT m Term
-
-/-- Assert a formula.
-
-- `term`: The formula to assert.
--/
-extern_def assertFormula : Term → SolverT m Unit
-
-/-- Check satisfiability. -/
-extern_def checkSat : SolverT m Result
-
-/-- Check satisfiability assuming the given formulas.
-
-- `assumptions`: The formulas to assume.
--/
-extern_def checkSatAssuming : (assumptions : Array Term) → SolverT m Result
-
-/-- Get a proof associated with the most recent call to `checkSat`.
-
-Requires to enable option `produce-proofs`.
--/
-extern_def getProof : SolverT m (Array Proof)
-
-/--
-Get the values of the given term in the current model.
-
-SMT-LIB:
-
-\verbatim embed:rst:leading-asterisk
-.. code:: smtlib
-
-    (get-value ( <term>* ))
-\endverbatim
-
-- `terms`: The term for which the value is queried.
--/
-extern_def getValue (term : Term) : SolverT m Term
-
-/--
-Get the values of the given terms in the current model.
-
-SMT-LIB:
-
-\verbatim embed:rst:leading-asterisk
-.. code:: smtlib
-
-    (get-value ( <term>* ))
-\endverbatim
-
-- `terms`: The terms for which the values are queried.
--/
-extern_def getValues (terms : Array Term) : SolverT m (Array Term)
-
-/-- Prints a proof as a string in a selected proof format mode.
-
-Other aspects of printing are taken from the solver options.
-
-- `proof`: A proof, usually obtained from `getProof`.
--/
-extern_def proofToString : Proof → SolverT m String
-
-/-- Parse a string containing SMT-LIB commands.
-
-Commands that produce a result such as `(check-sat)`, `(get-model)`, ... are executed but the
-results are ignored.
--/
-extern_def parseCommands : String → SolverT m Unit
-
-/-- Run a `query` given a term manager `tm`. -/
-def run (tm : TermManager) (query : SolverT m α) : m (Except Error α) :=
-  return match ← ExceptT.run query (new tm) with
-  | (.ok x, _) => .ok x
-  | (.error e, _) => .error e
-
-/-- Run a `query` given a term manager `tm`. -/
-def run! [Inhabited α] (tm : TermManager) (query : SolverT m α) : m α := do
-  match ← ExceptT.run query (new tm) with
-  | (.ok x, _) => return x
-  | (.error e, _) => do
-    panic! s!"{e}"
+end
 
 end Solver
 
-end cvc5
+
+
+/-! ## Environment operations -/
+
+
+
+namespace Env
+
+/-- Get the Boolean sort. -/
+@[extern "termManager_getBooleanSort"]
+private opaque getBooleanSort' : TermManager → Srt ω
+
+def getBooleanSort : Env ω (Srt ω) :=
+  Env.managerDo (return getBooleanSort' ·)
+
+end Env
+
+
+
+namespace Srt
+
+-- /-- The null sort. -/
+-- extern_def null : Unit → Srt ω
+
+-- instance : Inhabited (Srt ω) := ⟨null ()⟩
+
+-- /-- Comparison for structural equality. -/
+-- protected extern_def beq : (Srt ω) → (Srt ω) → Bool
+
+-- instance : BEq (Srt ω) := ⟨Srt.beq⟩
+
+-- /-- Less than comparison. -/
+-- protected extern_def blt : Srt ω → Srt ω → Bool
+
+-- /-- Greater than comparison. -/
+-- protected extern_def bgt : Srt ω → Srt ω → Bool
+
+-- /-- Less than or equal comparison. -/
+-- protected extern_def ble : Srt ω → Srt ω → Bool
+
+-- /-- Greater than or equal comparison. -/
+-- protected extern_def bge : Srt ω → Srt ω → Bool
+
+-- /-- Comparison of two sorts. -/
+-- protected def compare (s1 s2 : Srt ω) : Ordering :=
+--   if s1.beq s2 then .eq
+--   else if s1.bgt s2 then .gt
+--   else .lt
+
+-- instance : Ord (Srt ω) := ⟨Srt.compare⟩
+
+-- instance : LT (Srt ω) where
+--   lt := (Srt.blt · ·)
+
+-- instance : DecidableLT (Srt ω) :=
+--   fun s1 s2 => if h : s1.blt s2 then .isTrue h else .isFalse h
+
+-- instance : LE (Srt ω) where
+--   le := (Srt.ble · ·)
+
+-- instance : DecidableLE (Srt ω) :=
+--   fun s1 s2 => if h : s1.ble s2 then .isTrue h else .isFalse h
+
+-- /-- Hash function for cvc5 sorts. -/
+-- protected extern_def hash : Srt ω → UInt64
+
+-- instance : Hashable (Srt ω) := ⟨Srt.hash⟩
+
+-- /-- Get the kind of this sort. -/
+-- extern_def getKind : Srt ω → SortKind
+
+-- /-- Determine if this is the null sort (`Srt ω`). -/
+-- extern_def isNull : Srt ω → Bool
+
+-- /-- Determine if this is the Boolean sort (SMT-LIB: `Bool`). -/
+-- extern_def isBoolean : Srt ω → Bool
+
+-- /-- Determine if this is the Integer sort (SMT-LIB: `Int`). -/
+-- extern_def isInteger : Srt ω → Bool
+
+-- /-- Determine if this is the Real sort (SMT-LIB: `Real`). -/
+-- extern_def isReal : Srt ω → Bool
+
+-- /-- Determine if this is the String sort (SMT-LIB: `String`). -/
+-- extern_def isString : Srt ω → Bool
+
+-- /-- Determine if this is the regular expression sort (SMT-LIB: `RegLan`). -/
+-- extern_def isRegExp : Srt ω → Bool
+
+-- /-- Determine if this is the rounding mode sort (SMT-LIB: `RoundingMode`). -/
+-- extern_def isRoundingMode : Srt ω → Bool
+
+-- /-- Determine if this is a bit-vector sort (SMT-LIB: `(_ BitVec i)`). -/
+-- extern_def isBitVector : Srt ω → Bool
+
+-- /-- Determine if this is a floating-point sort (SMT-LIB: `(_ FloatingPoint eb sb)`). -/
+-- extern_def isFloatingPoint : Srt ω → Bool
+
+-- /-- Determine if this is a datatype sort. -/
+-- extern_def isDatatype : Srt ω → Bool
+
+-- /-- Determine if this is a datatype constructor sort. -/
+-- extern_def isDatatypeConstructor : Srt ω → Bool
+
+-- /-- Determine if this is a datatype selector sort. -/
+-- extern_def isDatatypeSelector : Srt ω → Bool
+
+-- /-- Determine if this is a datatype tester sort. -/
+-- extern_def isDatatypeTester : Srt ω → Bool
+
+-- /-- Determine if this is a datatype updater sort. -/
+-- extern_def isDatatypeUpdater : Srt ω → Bool
+
+-- /-- Determine if this is a function sort. -/
+-- extern_def isFunction : Srt ω → Bool
+
+-- /-- Determine if this is a predicate sort.
+
+-- A predicate sort is a function sort that maps to the Boolean sort. All predicate sorts are also
+-- function sorts.
+-- -/
+-- extern_def isPredicate : Srt ω → Bool
+
+-- /-- Determine if this is a tuple sort. -/
+-- extern_def isTuple : Srt ω → Bool
+
+-- /-- Determine if this is a nullable sort. -/
+-- extern_def isNullable : Srt ω → Bool
+
+-- /-- Determine if this is a record sort.
+
+-- **Warning**: this function is experimental and may change in future versions.
+-- -/
+-- extern_def isRecord : Srt ω → Bool
+
+-- /-- Determine if this is an array sort. -/
+-- extern_def isArray : Srt ω → Bool
+
+-- /-- Determine if this is a finite field sort. -/
+-- extern_def isFiniteField : Srt ω → Bool
+
+-- /-- Determine if this is a Set sort. -/
+-- extern_def isSet : Srt ω → Bool
+
+-- /-- Determine if this is a Bag sort. -/
+-- extern_def isBag : Srt ω → Bool
+
+-- /-- Determine if this is a Sequence sort. -/
+-- extern_def isSequence : Srt ω → Bool
+
+-- /-- Determine if this is an abstract sort. -/
+-- extern_def isAbstract : Srt ω → Bool
+
+-- /-- Determine if this is an uninterpreted sort. -/
+-- extern_def isUninterpretedSort : Srt ω → Bool
+
+-- /-- Determine if this is an uninterpreted sort constructor.
+
+-- An uninterpreted sort constructor has arity `> 0` and can be instantiated to construct uninterpreted
+-- sorts with given sort parameters.
+-- -/
+-- extern_def isUninterpretedSortConstructor : Srt ω → Bool
+
+-- /-- Determine if this is an instantiated (parametric datatype or uninterpreted sort constructor)
+-- sort.
+
+-- An instantiated sort is a sort that has been constructed from instantiating a sort with sort
+-- arguments --- see also `cvc5.Sort.instantiate`.
+-- -/
+-- extern_def isInstantiated : Srt ω → Bool
+
+-- /-- A string representation of this sort. -/
+-- protected extern_def toString : Srt ω → String
+
+-- /-- Determine if this term has a symbol (a name).
+
+-- For example, free constants and variables have symbols.
+-- -/
+-- extern_def!? hasSymbol : Srt ω → Except Error Bool
+
+-- /-- Get the symbol of this sort.
+
+-- The symbol of this sort is the string that was provided when constructing it *via* one of
+-- `Solver.mkUninterpretedSort`, `Solver.mkUnresolvedSort`, or
+-- `Solver.mkUninterpretedSortConstructorSort`.
+-- -/
+-- extern_def!? getSymbol : Srt ω → Except Error String
+
+-- /-- The arity of a function sort. -/
+-- extern_def!? getFunctionArity : Srt ω → Except Error Nat
+
+-- /-- The domain sorts of a function sort. -/
+-- extern_def!? getFunctionDomainSorts : Srt ω → Except Error (Array (Srt ω))
+
+-- /-- The codomain sort of a function sort. -/
+-- extern_def!? getFunctionCodomainSort : Srt ω → Except Error (Srt ω)
+
+-- /-- The array index sort of an array index. -/
+-- extern_def!? getArrayIndexSort : Srt ω → Except Error (Srt ω)
+
+-- /-- The array element sort of an array index. -/
+-- extern_def!? getArrayElementSort : Srt ω → Except Error (Srt ω)
+
+-- /-- The element sort of a set sort. -/
+-- extern_def!? getSetElementSort : Srt ω → Except Error (Srt ω)
+
+-- /-- The element sort of a bag sort. -/
+-- extern_def!? getBagElementSort : Srt ω → Except Error (Srt ω)
+
+-- /-- The element sort of a sequence sort. -/
+-- extern_def!? getSequenceElementSort : Srt ω → Except Error (Srt ω)
+
+-- /-- The sort kind of an abstract sort, which denotes the kind of sorts that this abstract sort
+-- denotes.
+-- -/
+-- extern_def!? getAbstractedKind : Srt ω → Except Error SortKind
+
+-- /-- The arity of an uninterpreted sort constructor sort. -/
+-- extern_def!? getUninterpretedSortConstructorArity : Srt ω → Except Error UInt32
+
+-- /-- The bit-width of the bit-vector sort. -/
+-- extern_def!? getBitVectorSize : Srt ω → Except Error UInt32
+
+-- /-- The size of the finite field sort. -/
+-- extern_def!? getFiniteFieldSize : Srt ω → Except Error Nat
+
+-- /-- The bit-width of the exponent of the floating-point sort. -/
+-- extern_def!? getFloatingPointExponentSize : Srt ω → Except Error UInt32
+
+-- /-- The width of the significand of the floating-point sort. -/
+-- extern_def!? getFloatingPointSignificandSize : Srt ω → Except Error UInt32
+
+-- /-- The length of a tuple sort. -/
+-- extern_def!? getTupleLength : Srt ω → Except Error UInt32
+
+-- /-- The element sorts of a tuple sort. -/
+-- extern_def!? getTupleSorts : Srt ω → Except Error (Array (Srt ω))
+
+-- /-- The element sort of a nullable sort. -/
+-- extern_def!? getNullableElementSort : Srt ω → Except Error (Srt ω)
+
+-- /-- Get the associated uninterpreted sort constructor of an instantiated uninterpreted sort. -/
+-- extern_def!? getUninterpretedSortConstructor : Srt ω → Except Error (Srt ω)
+
+-- /-- Instantiate a parameterized datatype sort or uninterpreted sort constructor sort.
+
+-- Create sort parameters with `TermManager.mkParamSort symbol`.
+
+-- - `params` The list of sort parameters to instantiate with.
+-- -/
+-- extern_def!? instantiate : Srt ω → (params : Array (Srt ω)) → Except Error (Srt ω)
+
+-- /-- Simultaneous substitution of Sorts.
+
+-- Note that this replacement is applied during a pre-order traversal and only once to the sort. It is not run until fix point. In the case that `sorts` contains duplicates, the replacement earliest in
+-- the vector takes priority.
+
+-- **Warning:** This function is experimental and may change in future versions.
+
+-- - `sorts` The sub-sorts to be substituted within this sort.
+-- - `replacements` The sort replacing the substituted sub-sorts.
+-- -/
+-- extern_def!? substitute
+-- : Srt ω → (sorts : Array (Srt ω)) → (replacements : Array (Srt ω)) → Except Error (Srt ω)
+
+-- instance : ToString (Srt ω) := ⟨Srt.toString⟩
+-- instance : Repr (Srt ω) := ⟨fun self _ => self.toString⟩
+
+-- end Srt
+
+
+
+-- private opaque OpImpl : NonemptyType.{0}
+
+-- /-- A cvc5 operator.
+
+-- An operator is a term that represents certain operators, instantiated with its required parameters,
+-- *e.g.*, a `Term` of kind `Kind.BITVECTOR_EXTRACT`.
+-- -/
+-- @[irreducible]
+-- def Op : (ω : Type) → Type := fun _ => OpImpl.type
+
+-- namespace Op
+
+-- private theorem typeDef : Op ω = OpImpl.type :=
+--   by unfold Op ; rfl
+
+-- private def toImpl : Op ω → OpImpl.type :=
+--   by rw [typeDef] ; exact id
+
+-- private def ofImpl : OpImpl.type → Op ω :=
+--   by rw [typeDef] ; exact id
+
+-- instance : Nonempty (Op ω) :=
+--   by rw [typeDef] ; exact OpImpl.property
+
+-- /-- The null operator. -/
+-- extern_def null : Unit → Op ω
+
+-- instance : Inhabited Op := ⟨null ()⟩
+
+-- /-- Syntactic equality operator. -/
+-- protected extern_def beq : Op → Op → Bool
+
+-- instance : BEq Op := ⟨Op.beq⟩
+
+-- /-- Get the kind of this operator. -/
+-- extern_def getKind : Op → Kind
+
+-- /-- Determine if this operator is nullary. -/
+-- extern_def isNull : Op → Bool
+
+-- /-- Determine if this operator is indexed. -/
+-- extern_def isIndexed : Op → Bool
+
+-- /-- Get the number of indices of this operator. -/
+-- extern_def getNumIndices : Op → Nat
+
+-- /-- Get the index at position `i` of an indexed operator. -/
+-- protected extern_def get : (op : Op) → Fin op.getNumIndices → Term ω
+
+-- /-- Get the string representation of this operator. -/
+-- protected extern_def toString : Op → String
+
+-- instance {ω : outParam Type} : GetElem Op Nat (Term ω) fun op i => i < op.getNumIndices where
+--   getElem op i h := op.get ⟨i, h⟩
+
+-- instance : ToString Op := ⟨Op.toString⟩
+
+-- end Op
+
+-- namespace Term
+
+-- /-- The null term. -/
+-- extern_def null : Unit → Term
+
+-- instance : Inhabited Term := ⟨null ()⟩
+
+-- /-- Syntactic equality operator. -/
+-- protected extern_def beq : Term → Term → Bool
+
+-- instance : BEq Term := ⟨Term.beq⟩
+
+-- protected extern_def hash : Term → UInt64
+
+-- instance : Hashable Term := ⟨Term.hash⟩
+
+-- /-- Determine if this term is nullary. -/
+-- extern_def isNull : Term → Bool
+
+-- /-- Get the kind of this term. -/
+-- extern_def getKind : Term → Kind
+
+-- /-- Get the sort of this term. -/
+-- extern_def getSort : Term → cvc5.Sort
+
+-- /-- Determine if this term has an operator. -/
+-- extern_def hasOp : Term → Bool
+
+-- /-- Determine if this term has a symbol (a name).
+
+-- For example, free constants and variables have symbols.
+-- -/
+-- extern_def hasSymbol : Term → Bool
+
+-- /-- Get the id of this term. -/
+-- extern_def getId : Term → Nat
+
+-- /-- Get the number of children of this term. -/
+-- extern_def getNumChildren : Term → Nat
+
+-- /-- Is this term a skolem? -/
+-- extern_def isSkolem : Term → Bool
+
+-- /-- Get the child term of this term at a given index. -/
+-- protected extern_def get : (t : Term) → Fin t.getNumChildren → Term
+
+-- /-- Get the operator of a term with an operator.
+
+-- Requires that this term has an operator (see `hasOp`).
+-- -/
+-- extern_def!? getOp : Term → Except Error Op
+
+-- /-- Get the value of a Boolean term as a native Boolean value.
+
+-- Requires `term` to have sort Bool.
+-- -/
+-- extern_def!? getBooleanValue : Term → Except Error Bool
+
+-- /-- Get the string representation of a bit-vector value.
+
+-- Requires `term` to have a bit-vector sort.
+
+-- - `base`: `2` for binary, `10` for decimal, and `16` for hexadecimal.
+-- -/
+-- extern_def!? getBitVectorValue : Term → UInt32 → Except Error String
+
+-- /-- Get the native integral value of an integral value. -/
+-- extern_def!? getIntegerValue : Term → Except Error Int
+
+-- /-- Get the native rational value of a real, rational-compatible value. -/
+-- extern_def!? getRationalValue : Term → Except Error Std.Internal.Rat
+
+-- /-- Get the symbol of this term.
+
+-- Requires that this term has a symbol (see `hasSymbol`).
+
+-- The symbol of the term is the string that was provided when constructing it *via*
+-- `TermManager.mkConst` or `TermManager.mkVar`.
+-- -/
+-- extern_def!? getSymbol : Term → Except Error String
+
+-- /-- Get skolem identifier of this term.
+
+-- Requires `isSkolem`.
+-- -/
+-- extern_def!? getSkolemId : Term → Except Error SkolemId
+
+-- /-- Get the skolem indices of this term.
+
+-- Requires `isSkolem`.
+
+-- Returns the skolem indices of this term. This is a list of terms that the skolem function is indexed
+-- by. For example, the array diff skolem `SkolemId.ARRAY_DEQ_DIFF` is indexed by two arrays.
+-- -/
+-- extern_def!? getSkolemIndices : Term → Except Error (Array Term)
+
+-- instance : GetElem Term Nat Term fun t i => i < t.getNumChildren where
+--   getElem t i h := t.get ⟨i, h⟩
+
+-- protected def forIn {β : Type u} [Monad m] (t : Term) (b : β) (f : Term → β → m (ForInStep β)) : m β :=
+--   let rec loop (i : Nat) (h : i ≤ t.getNumChildren) (b : β) : m β := do
+--     match i, h with
+--     | 0,   _ => pure b
+--     | i+1, h =>
+--       have h' : i < t.getNumChildren := Nat.lt_of_lt_of_le (Nat.lt_succ_self i) h
+--       have : t.getNumChildren - 1 < t.getNumChildren := Nat.sub_lt (Nat.zero_lt_of_lt h') (by decide)
+--       have : t.getNumChildren - 1 - i < t.getNumChildren := Nat.lt_of_le_of_lt (Nat.sub_le (t.getNumChildren - 1) i) this
+--       match (← f t[t.getNumChildren - 1 - i] b) with
+--       | ForInStep.done b  => pure b
+--       | ForInStep.yield b => loop i (Nat.le_of_lt h') b
+--   loop t.getNumChildren (Nat.le_refl _) b
+
+-- instance : ForIn m Term Term where
+--   forIn := Term.forIn
+
+-- /-- Get the children of a term. -/
+-- def getChildren (t : Term) : Array Term := Id.run do
+--   let mut cts := #[]
+--   for ct in t do
+--     cts := cts.push ct
+--   cts
+
+-- /-- Boolean negation. -/
+-- protected extern_def!? not : (t : Term) → Except Error Term
+
+-- /-- Boolean and. -/
+-- protected extern_def!? and : (lft rgt : Term) → Except Error Term
+
+-- /-- Boolean or. -/
+-- protected extern_def!? or : (lft rgt : Term) → Except Error Term
+
+-- /-- Boolean exclusive or. -/
+-- protected extern_def!? xor : (lft rgt : Term) → Except Error Term
+
+-- /-- Equality. -/
+-- protected extern_def!? eq : (lft rgt : Term) → Except Error Term
+
+-- /-- Boolean implication. -/
+-- protected extern_def!? imp : (lft rgt : Term) → Except Error Term
+
+-- /-- If-then-else.
+
+-- - `cnd`: condition, must be a Boolean term;
+-- - `thn`: then-branch of some sort `S`;
+-- - `els`: else-branch of *the same* sort `S`.
+-- -/
+-- protected extern_def!? ite : (cnd thn els : Term) → Except Error Term
+
+-- /-- A string representation of this term. -/
+-- protected extern_def toString : Term → String
+
+-- instance : ToString Term := ⟨Term.toString⟩
+
+-- end Term
+
+-- namespace Proof
+
+-- /-- The null proof. -/
+-- extern_def null : Unit → Proof
+
+-- instance : Inhabited Proof := ⟨null ()⟩
+
+-- /-- Get the proof rule used by the root step of the root. -/
+-- extern_def getRule : Proof → ProofRule
+
+-- /-- Get the proof rewrite rule used by the root step of the proof.
+
+-- Requires that `getRule` does not return `ProofRule.DSL_REWRITE` or `ProofRule.REWRITE`.
+-- -/
+-- extern_def!? getRewriteRule : Proof → Except Error ProofRewriteRule
+
+-- /-- The conclusion of the root step of the proof. -/
+-- extern_def getResult : Proof → Term
+
+-- /-- The premises of the root step of the proof. -/
+-- extern_def getChildren : Proof → Array Proof
+
+-- /-- The arguments of the root step of the proof as a vector of terms.
+
+-- Some of those terms might be strings.
+-- -/
+-- extern_def getArguments : Proof → Array Term
+
+-- /-- Operator overloading for referential equality of two proofs. -/
+-- protected extern_def beq : Proof → Proof → Bool
+
+-- instance : BEq Proof := ⟨Proof.beq⟩
+
+-- /-- Hash function for proofs. -/
+-- protected extern_def hash : Proof → UInt64
+
+-- instance : Hashable Proof := ⟨Proof.hash⟩
+
+-- end Proof
+
+-- namespace TermManager
+
+-- /-- Constructor. -/
+-- extern_def new : BaseIO TermManager
+
+-- /-- Get the Boolean sort. -/
+-- extern_def getBooleanSort : TermManager → cvc5.Sort
+
+-- /-- Get the Integer sort. -/
+-- extern_def getIntegerSort : TermManager → cvc5.Sort
+
+-- /-- Get the Real sort. -/
+-- extern_def getRealSort : TermManager → cvc5.Sort
+
+-- /-- Get the regular expression sort. -/
+-- extern_def getRegExpSort : TermManager → cvc5.Sort
+
+-- /-- Get the rounding mode sort. -/
+-- extern_def getRoundingModeSort : TermManager → cvc5.Sort
+
+-- /-- Get the string sort. -/
+-- extern_def getStringSort : TermManager → cvc5.Sort
+
+-- /-- Create an array sort.
+
+-- - `indexSort` The array index sort.
+-- - `elemSort` The array element sort.
+-- -/
+-- extern_def!? mkArraySort : TermManager → (indexSort elemSort : cvc5.Sort) → Except Error cvc5.Sort
+
+-- /-- Create a bit-vector sort.
+
+-- - `size` The bit-width of the bit-vector sort.
+-- -/
+-- extern_def!? mkBitVectorSort : TermManager → (size : UInt32) → Except Error cvc5.Sort
+
+-- /-- Create a floating-point sort.
+
+-- - `exp` The bit-width of the exponent of the floating-point sort.
+-- - `sig` The bit-width of the significand of the floating-point sort.
+-- -/
+-- extern_def!? mkFloatingPointSort : TermManager → (exp sig : UInt32) → Except Error cvc5.Sort
+
+-- /-- Create a finite-field sort from a given string of base n.
+
+-- - `size` The modulus of the field. Must be a prime.
+-- -/
+-- private extern_def mkFiniteFieldSortFromString : TermManager → (size : String) → (base : UInt32 := 10) → Except Error cvc5.Sort
+
+-- @[inherit_doc mkFiniteFieldSortFromString]
+-- abbrev mkFiniteFieldSort (tm : TermManager) : (size : Nat) → Except Error cvc5.Sort :=
+--   (tm.mkFiniteFieldSortFromString · 10) ∘ toString
+-- @[inherit_doc mkFiniteFieldSortFromString]
+-- abbrev mkFiniteFieldSort! (tm : TermManager) : (size : Nat) → cvc5.Sort :=
+--   Error.unwrap! ∘ (tm.mkFiniteFieldSortFromString · 10) ∘ toString
+-- @[inherit_doc mkFiniteFieldSortFromString]
+-- abbrev mkFiniteFieldSort? (tm : TermManager) : (size : Nat) → Option cvc5.Sort :=
+--   Except.toOption ∘ (tm.mkFiniteFieldSortFromString · 10) ∘ toString
+
+-- /-- Create function sort.
+
+-- - `sorts` The sort of the function arguments.
+-- - `codomain` The sort of the function return value.
+-- -/
+-- extern_def!? mkFunctionSort
+-- : TermManager → (sorts : Array cvc5.Sort) → (codomain : cvc5.Sort) → Except Error cvc5.Sort
+
+-- /-- Create a predicate sort.
+
+-- This is equivalent to calling `mkFunctionSort` with Boolean sort as the codomain.
+
+-- - `sorts` The list of sorts of the predicate.
+-- -/
+-- extern_def!? mkPredicateSort : TermManager → (sorts : Array cvc5.Sort) → Except Error cvc5.Sort
+
+-- /-- Create a tuple sort.
+
+-- - `sorts` The sorts of the elements of the tuple.
+-- -/
+-- extern_def!? mkTupleSort : TermManager → (sorts : Array cvc5.Sort) → Except Error cvc5.Sort
+
+-- /-- Create an uninterpreted sort constructor sort.
+
+-- An uninterpreted sort constructor is an uninterpreted sort with arity > 0.
+
+-- - `arity` The arity of the sort (must be > 0).
+-- - `symbol` The symbol of the sort.
+-- -/
+-- extern_def!? mkUninterpretedSortConstructorSort
+-- : TermManager → (arity : Nat) → (symbol : String) → Except Error cvc5.Sort
+
+-- /-- Create a set parameter.
+
+-- - `elemSort` The sort of the set elements.
+-- -/
+-- extern_def!? mkSetSort : TermManager → (sort : cvc5.Sort) → Except Error cvc5.Sort
+
+-- /-- Create a set parameter.
+
+-- - `elemSort` The sort of the set elements.
+-- -/
+-- extern_def!? mkBagSort : TermManager → (sort : cvc5.Sort) → Except Error cvc5.Sort
+
+-- /-- Create a set parameter.
+
+-- - `elemSort` The sort of the set elements.
+-- -/
+-- extern_def!? mkSequenceSort : TermManager → (sort : cvc5.Sort) → Except Error cvc5.Sort
+
+-- /-- Create an abstract sort. An abstract sort represents a sort for a given kind whose parameters
+-- and arguments are unspecified.
+
+-- The kind `k` must be the kind of a sort that can be abstracted, *i.e.* a sort that has indices or
+-- arguments sorts. For example, `SortKind.ARRAY_SORT` and `SortKind.BITVECTOR_SORT` can be passed as
+-- the kind `k` to this function, while `SortKind.INTEGER_SORT` and `SortKind.STRING_SORT` cannot.
+
+-- **NB:** Providing the kind `SortKind.ABSTRACT_SORT` as an argument to this function returns the
+-- (fully) unspecified sort, denoted `?`.
+
+-- **NB:** Providing a kind `k` that has no indices and a fixed arity of argument sorts will return the
+-- sort of kind `k` whose arguments are the unspecified sort. For example, `mkAbstractSort
+-- SortKind.ARRAY_SORT` will return the sort `(ARRAY_SORT ? ?)` instead of the abstract sort whose
+-- abstract kind is `SortKind.ARRAY_SORT`.
+-- -/
+-- extern_def!? mkAbstractSort : TermManager → (k : SortKind) → Except Error cvc5.Sort
+
+-- /-- Create an uninterpreted sort.
+
+-- - `symbol` The name of the sort.
+-- -/
+-- extern_def mkUninterpretedSort : TermManager → (symbol : String) → cvc5.Sort
+
+-- /-- Create a nullable sort.
+
+-- - `sort` The sort of the element of the nullable.
+-- -/
+-- extern_def!? mkNullableSort : TermManager → (sort : cvc5.Sort) → Except Error cvc5.Sort
+
+-- /-- Create a sort parameter.
+
+-- - `symbol` The name of the sort.
+
+-- **Warning**: This function is experimental and may change in future versions.
+-- -/
+-- extern_def mkParamSort : TermManager → (symbol : String) → cvc5.Sort
+
+-- /-- Create a Boolean constant.
+
+-- - `b`: The Boolean constant.
+-- -/
+-- extern_def mkBoolean : TermManager → (b : Bool) → Term
+
+-- /-- Create an integer-value term.
+
+-- - `s`: the string representation of the constant, may represent an integer such as (`"123"`).
+-- -/
+-- private extern_def mkIntegerFromString : TermManager → (s : String) → Except Error Term
+-- with
+--   /-- Create an integer-value term. -/
+--   mkInteger (tm : TermManager) : Int → Term :=
+--     Error.unwrap! ∘ tm.mkIntegerFromString ∘ toString
+
+-- /-- Create a real-value term.
+
+-- - `s`: the string representation of the constant, may represent an integer (`"123"`) or a real
+--   constant (`"12.34"`, `"12/34"`).
+-- -/
+-- private extern_def mkRealFromString : TermManager → (s : String) → Except Error Term
+-- with
+--   /-- Create a real-value term from a `Std.Internal.Rat`. -/
+--   mkRealOfRat (tm : TermManager) (rat : Std.Internal.Rat) : Term :=
+--     tm.mkRealFromString s!"{rat.num}/{rat.den}" |> Error.unwrap!
+--   /-- Create a real-value term from numerator/denominator `Int`-s. -/
+--   mkReal (tm : TermManager)
+--     (num : Int) (den : Int := 1) (den_ne_0 : den ≠ 0 := by simp <;> omega)
+--   : Term :=
+--     let (num, den) :=
+--       match h : den with
+--       | .ofNat 0 => by contradiction
+--       | .ofNat den => (num, den)
+--       | .negSucc denMinus1 => (-num, denMinus1.succ)
+--     tm.mkRealOfRat <| Std.Internal.mkRat num den
+
+-- /-- Create operator of Kind:
+
+-- - `Kind.BITVECTOR_EXTRACT`
+-- - `Kind.BITVECTOR_REPEAT`
+-- - `Kind.BITVECTOR_ROTATE_LEFT`
+-- - `Kind.BITVECTOR_ROTATE_RIGHT`
+-- - `Kind.BITVECTOR_SIGN_EXTEND`
+-- - `Kind.BITVECTOR_ZERO_EXTEND`
+-- - `Kind.DIVISIBLE`
+-- - `Kind.FLOATINGPOINT_TO_FP_FROM_FP`
+-- - `Kind.FLOATINGPOINT_TO_FP_FROM_IEEE_BV`
+-- - `Kind.FLOATINGPOINT_TO_FP_FROM_REAL`
+-- - `Kind.FLOATINGPOINT_TO_FP_FROM_SBV`
+-- - `Kind.FLOATINGPOINT_TO_FP_FROM_UBV`
+-- - `Kind.FLOATINGPOINT_TO_SBV`
+-- - `Kind.FLOATINGPOINT_TO_UBV`
+-- - `Kind.INT_TO_BITVECTOR`
+-- - `Kind.TUPLE_PROJECT`
+
+-- See `cvc5.Kind` for a description of the parameters.
+
+-- - `kind` The kind of the operator.
+-- - `args` The arguments (indices) of the operator.
+
+-- If `args` is empty, the `Op` simply wraps the `cvc5.Kind`. The `Kind` can be used in
+-- `Solver.mkTerm` directly without creating an `Op` first.
+-- -/
+-- extern_def!? mkOpOfIndices : TermManager → (kind : Kind) → (args : Array Nat := #[]) → Except Error Op
+
+-- @[inherit_doc mkOpOfIndices]
+-- abbrev mkOp := @mkOpOfIndices
+-- @[inherit_doc mkOpOfIndices!]
+-- abbrev mkOp! := @mkOpOfIndices!
+-- @[inherit_doc mkOpOfIndices?]
+-- abbrev mkOp? := @mkOpOfIndices?
+
+-- /-- Create operator of kind:
+
+-- - `Kind.DIVISIBLE` (to support arbitrary precision integers)
+
+-- See `cvc5.Kind` for a description of the parameters.
+
+-- - `kind` The kind of the operator.
+-- - `arg` The string argument to this operator.
+-- -/
+-- extern_def!? mkOpOfString : TermManager → (kind : Kind) → (arg : String) → Except Error Op
+
+-- /-- Create n-ary term of given kind.
+
+-- - `kind` The kind of the term.
+-- - `children` The children of the term.
+-- -/
+-- extern_def!? mkTerm : TermManager → (kind : Kind) → (children : Array Term := #[]) → Except Error Term
+
+-- /-- Create n-ary term of given kind from a given operator.
+
+-- Create operators with `mkOp`.
+
+-- - `op` The operator.
+-- - `children` The children of the term.
+-- -/
+-- extern_def!? mkTermOfOp : TermManager → (op : Op) → (children : Array Term := #[]) → Except Error Term
+
+-- /-- **THIS FUNCTION MUST NOT BE EXPOSED.**
+
+-- **It produces a different (fresh) term every time it's called which is really bad for purity.**
+
+-- Create a free constant.
+
+-- Note that the returned term is always fresh, even if the same arguments were provided on a
+-- previous call to `mkConst`.
+
+-- - `sort` The sort of the constant.
+-- - `symbol` The name of the constant (optional).
+-- -/
+-- private
+-- def mkConst (_ : TermManager) (_ : cvc5.Sort) (_ : String := "") : Term :=
+--   panic! "illegal call to `cvc5.TermManager.mkConst"
+
+-- end TermManager
+
+-- namespace Solver
+
+-- variable [Monad m]
+
+-- /-- Only used by FFI to wrap *success* results. -/
+-- @[export solver_val]
+-- private def val (a : α) : SolverT m α := pure a
+
+-- /-- Only used by FFI to wrap errors. -/
+-- @[export solver_err]
+-- private def err (e : Error) : SolverT m α := throw e
+
+-- /-- Only used by FFI to wrap cvc5 errors. -/
+-- @[export solver_errOfString]
+-- private def errorOfString (msg : String) : SolverT m α := throw (.error msg)
+
+-- /-- Constructor.
+
+-- Constructs solver instance from a given term manager instance.
+
+-- - `tm`: The associated term manager.
+-- -/
+-- private extern_def new : TermManager → Solver
+
+-- /-- Get a string representation of the version of this solver. -/
+-- extern_def getVersion : SolverT m String
+
+-- /-- Set option.
+
+-- - `option`: The option name.
+-- - `value`: The option value.
+-- -/
+-- extern_def setOption (option value : String) : SolverT m Unit
+
+-- /-- Remove all assertions. -/
+-- extern_def resetAssertions : SolverT m Unit
+
+-- /-- Set logic.
+
+-- - `logic`: The logic to set.
+-- -/
+-- extern_def setLogic : (logic : String) → SolverT m Unit
+
+-- /-- Simplify a term or formula based on rewriting and (optionally) applying substitutions for
+-- solved variables.
+
+-- If `applySubs` is true, then for example, if `(= x 0)` was asserted to this solver, this function
+-- may replace occurrences of `x` with `0`.
+
+-- - `t` The term to simplify.
+-- - `applySubs` True to apply substitutions for solved variables.
+-- -/
+-- extern_def simplify : (term : Term) → (applySubs : Bool := false) → SolverT m Term
+
+-- /--
+-- Declare n-ary function symbol.
+
+-- SMT-LIB:
+
+-- \verbatim embed:rst:leading-asterisk
+--  .. code:: smtlib
+
+--      (declare-fun <symbol> ( <sort>* ) <sort>)
+--  \endverbatim
+
+-- - `symbol`: The name of the function.
+-- - `sorts`: The sorts of the parameters to this function.
+-- - `sort`: The sort of the return value of this function.
+-- - `fresh`: If true, then this method always returns a new Term. Otherwise, this method will always
+--   return the same Term for each call with the given sorts and symbol where fresh is false.
+-- -/
+-- extern_def declareFun (symbol : String) (sorts : Array cvc5.Sort) (sort : cvc5.Sort) (fresh := true) : SolverT m Term
+
+-- /-- Assert a formula.
+
+-- - `term`: The formula to assert.
+-- -/
+-- extern_def assertFormula : Term → SolverT m Unit
+
+-- /-- Check satisfiability. -/
+-- extern_def checkSat : SolverT m Result
+
+-- /-- Check satisfiability assuming the given formulas.
+
+-- - `assumptions`: The formulas to assume.
+-- -/
+-- extern_def checkSatAssuming : (assumptions : Array Term) → SolverT m Result
+
+-- /-- Get a proof associated with the most recent call to `checkSat`.
+
+-- Requires to enable option `produce-proofs`.
+-- -/
+-- extern_def getProof : SolverT m (Array Proof)
+
+-- /--
+-- Get the values of the given term in the current model.
+
+-- SMT-LIB:
+
+-- \verbatim embed:rst:leading-asterisk
+-- .. code:: smtlib
+
+--     (get-value ( <term>* ))
+-- \endverbatim
+
+-- - `terms`: The term for which the value is queried.
+-- -/
+-- extern_def getValue (term : Term) : SolverT m Term
+
+-- /--
+-- Get the values of the given terms in the current model.
+
+-- SMT-LIB:
+
+-- \verbatim embed:rst:leading-asterisk
+-- .. code:: smtlib
+
+--     (get-value ( <term>* ))
+-- \endverbatim
+
+-- - `terms`: The terms for which the values are queried.
+-- -/
+-- extern_def getValues (terms : Array Term) : SolverT m (Array Term)
+
+-- /-- Prints a proof as a string in a selected proof format mode.
+
+-- Other aspects of printing are taken from the solver options.
+
+-- - `proof`: A proof, usually obtained from `getProof`.
+-- -/
+-- extern_def proofToString : Proof → SolverT m String
+
+-- /-- Parse a string containing SMT-LIB commands.
+
+-- Commands that produce a result such as `(check-sat)`, `(get-model)`, ... are executed but the
+-- results are ignored.
+-- -/
+-- extern_def parseCommands : String → SolverT m Unit
+
+-- /-- Run a `query` given a term manager `tm`. -/
+-- def run (tm : TermManager) (query : SolverT m α) : m (Except Error α) :=
+--   return match ← ExceptT.run query (new tm) with
+--   | (.ok x, _) => .ok x
+--   | (.error e, _) => .error e
+
+-- /-- Run a `query` given a term manager `tm`. -/
+-- def run! [Inhabited α] (tm : TermManager) (query : SolverT m α) : m α := do
+--   match ← ExceptT.run query (new tm) with
+--   | (.ok x, _) => return x
+--   | (.error e, _) => do
+--     panic! s!"{e}"
+
+-- end Solver
+
+-- end cvc5
