cvc5/Cvc.lean
@@ -1,0 +1,1295 @@
+/-
+Copyright (c) 2023-2024 by the authors listed in the file AUTHORS and their
+institutional affiliations. All rights reserved.
+Released under Apache 2.0 license as described in the file LICENSE.
+Authors: Abdalrhman Mohamed, Adrien Champion
+-/
+
+import Std.Internal.Rat
+
+import cvc5.Init
+import cvc5.Kind
+import cvc5.ProofRule
+import cvc5.SkolemId
+import cvc5.Types
+
+namespace cvc5
+
+namespace Kind
+
+/-- Produces a string representation. -/
+@[extern "kind_toString"]
+protected opaque toString : Kind → String
+
+instance : ToString Kind := ⟨Kind.toString⟩
+
+/-- Produces a hash. -/
+@[extern "kind_hash"]
+protected opaque hash : Kind → UInt64
+
+instance : Hashable Kind := ⟨Kind.hash⟩
+
+end Kind
+
+namespace SortKind
+
+/-- Produces a string representation. -/
+@[extern "sortKind_toString"]
+protected opaque toString : SortKind → String
+
+instance : ToString SortKind := ⟨SortKind.toString⟩
+
+/-- Produces a hash. -/
+@[extern "sortKind_hash"]
+protected opaque hash : SortKind → UInt64
+
+instance : Hashable SortKind := ⟨SortKind.hash⟩
+
+end SortKind
+
+namespace ProofRule
+
+/-- Produces a string representation. -/
+@[extern "proofRule_toString"]
+protected opaque toString : ProofRule → String
+
+instance : ToString ProofRule := ⟨ProofRule.toString⟩
+
+/-- Produces a hash. -/
+@[extern "proofRule_hash"]
+protected opaque hash : ProofRule → UInt64
+
+instance : Hashable ProofRule := ⟨ProofRule.hash⟩
+
+end ProofRule
+
+namespace SkolemId
+
+/-- Produces a string representation. -/
+@[extern "skolemId_toString"]
+protected opaque toString : SkolemId → String
+
+instance : ToString SkolemId := ⟨SkolemId.toString⟩
+
+/-- Produces a hash. -/
+@[extern "skolemId_hash"]
+protected opaque hash : SkolemId → UInt64
+
+instance : Hashable SkolemId := ⟨SkolemId.hash⟩
+
+end SkolemId
+
+namespace ProofRewriteRule
+
+/-- Produces a string representation. -/
+@[extern "proofRewriteRule_toString"]
+protected opaque toString : ProofRewriteRule → String
+
+instance : ToString ProofRewriteRule := ⟨ProofRewriteRule.toString⟩
+
+/-- Produces a hash. -/
+@[extern "proofRewriteRule_hash"]
+protected opaque hash : ProofRewriteRule → UInt64
+
+instance : Hashable ProofRewriteRule := ⟨ProofRewriteRule.hash⟩
+
+end ProofRewriteRule
+
+namespace UnknownExplanation
+
+/-- Produces a string representation. -/
+@[extern "unknownExplanation_toString"]
+protected opaque toString : UnknownExplanation → String
+
+instance : ToString UnknownExplanation := ⟨UnknownExplanation.toString⟩
+
+/-- Produces a hash. -/
+@[extern "unknownExplanation_hash"]
+protected opaque hash : UnknownExplanation → UInt64
+
+instance : Hashable UnknownExplanation := ⟨UnknownExplanation.hash⟩
+
+end UnknownExplanation
+
+namespace RoundingMode
+
+/-- Produces a string representation. -/
+@[extern "roundingMode_toString"]
+protected opaque toString : RoundingMode → String
+
+instance : ToString RoundingMode := ⟨RoundingMode.toString⟩
+
+/-- Produces a hash. -/
+@[extern "roundingMode_hash"]
+protected opaque hash : RoundingMode → UInt64
+
+instance : Hashable RoundingMode := ⟨RoundingMode.hash⟩
+
+end RoundingMode
+
+namespace BlockModelsMode
+
+/-- Produces a string representation. -/
+@[extern "blockModelsMode_toString"]
+protected opaque toString : BlockModelsMode → String
+
+instance : ToString BlockModelsMode := ⟨BlockModelsMode.toString⟩
+
+/-- Produces a hash. -/
+@[extern "blockModelsMode_hash"]
+protected opaque hash : BlockModelsMode → UInt64
+
+instance : Hashable BlockModelsMode := ⟨BlockModelsMode.hash⟩
+
+end BlockModelsMode
+
+namespace LearnedLitType
+
+/-- Produces a string representation. -/
+@[extern "learnedLitType_toString"]
+protected opaque toString : LearnedLitType → String
+
+instance : ToString LearnedLitType := ⟨LearnedLitType.toString⟩
+
+/-- Produces a hash. -/
+@[extern "learnedLitType_hash"]
+protected opaque hash : LearnedLitType → UInt64
+
+instance : Hashable LearnedLitType := ⟨LearnedLitType.hash⟩
+
+end LearnedLitType
+
+namespace ProofComponent
+
+/-- Produces a string representation. -/
+@[extern "proofComponent_toString"]
+protected opaque toString : ProofComponent → String
+
+instance : ToString ProofComponent := ⟨ProofComponent.toString⟩
+
+/-- Produces a hash. -/
+@[extern "proofComponent_hash"]
+protected opaque hash : ProofComponent → UInt64
+
+instance : Hashable ProofComponent := ⟨ProofComponent.hash⟩
+
+end ProofComponent
+
+namespace ProofFormat
+
+/-- Produces a string representation. -/
+@[extern "proofFormat_toString"]
+protected opaque toString : ProofFormat → String
+
+instance : ToString ProofFormat := ⟨ProofFormat.toString⟩
+
+/-- Produces a hash. -/
+@[extern "proofFormat_hash"]
+protected opaque hash : ProofFormat → UInt64
+
+instance : Hashable ProofFormat := ⟨ProofFormat.hash⟩
+
+end ProofFormat
+
+namespace FindSynthTarget
+
+/-- Produces a string representation. -/
+@[extern "findSynthTarget_toString"]
+protected opaque toString : FindSynthTarget → String
+
+instance : ToString FindSynthTarget := ⟨FindSynthTarget.toString⟩
+
+/-- Produces a hash. -/
+@[extern "findSynthTarget_hash"]
+protected opaque hash : FindSynthTarget → UInt64
+
+instance : Hashable FindSynthTarget := ⟨FindSynthTarget.hash⟩
+
+end FindSynthTarget
+
+namespace InputLanguage
+
+/-- Produces a string representation. -/
+@[extern "inputLanguage_toString"]
+protected opaque toString : InputLanguage → String
+
+instance : ToString InputLanguage := ⟨InputLanguage.toString⟩
+
+/-- Produces a hash. -/
+@[extern "inputLanguage_hash"]
+protected opaque hash : InputLanguage → UInt64
+
+instance : Hashable InputLanguage := ⟨InputLanguage.hash⟩
+
+end InputLanguage
+
+private opaque ResultImpl : NonemptyType.{0}
+
+/-- Encapsulation of a three-valued solver result, with explanations. -/
+def Result : Type := ResultImpl.type
+
+instance Result.instNonemptyResult : Nonempty Result := ResultImpl.property
+
+private opaque SortImpl : NonemptyType.{0}
+
+end cvc5
+
+/-- The sort of a cvc5 term. -/
+def cvc5.Sort : Type := cvc5.SortImpl.type
+
+namespace cvc5
+
+instance Sort.instNonemptySort : Nonempty cvc5.Sort := SortImpl.property
+
+private opaque OpImpl : NonemptyType.{0}
+
+/-- A cvc5 operator.
+
+An operator is a term that represents certain operators, instantiated with its required parameters,
+*e.g.*, a `Term` of kind `Kind.BITVECTOR_EXTRACT`.
+-/
+def Op : Type := OpImpl.type
+
+instance Op.instNonemptyOp : Nonempty Op := OpImpl.property
+
+private opaque TermImpl : NonemptyType.{0}
+
+/-- A cvc5 term. -/
+def Term : Type := TermImpl.type
+
+instance Term.instNonemptyTerm : Nonempty Term := TermImpl.property
+
+private opaque ProofImpl : NonemptyType.{0}
+
+/-- A cvc5 proof.
+
+Proofs are trees and every proof object corresponds to the root step of a proof. The branches of the
+root step are the premises of the step.
+-/
+def Proof : Type := ProofImpl.type
+
+instance Proof.instNonemptyProof : Nonempty Proof := ProofImpl.property
+
+private opaque TermManagerImpl : NonemptyType.{0}
+
+/-- Manager for cvc5 terms. -/
+def TermManager : Type := TermManagerImpl.type
+
+instance TermManager.instNonemptyTermManager : Nonempty TermManager := TermManagerImpl.property
+
+/-- Error type. -/
+inductive Error where
+  | missingValue
+  | error (msg : String)
+  | recoverable (msg : String)
+  | unsupported (msg : String)
+  | option (msg : String)
+deriving Repr
+
+private opaque SolverImpl : NonemptyType.{0}
+
+/-- A cvc5 solver. -/
+def Solver : Type := SolverImpl.type
+
+instance Solver.instNonemptySolver : Nonempty Solver := SolverImpl.property
+
+/-- Solver error/state-monad transformer. -/
+abbrev SolverT m := ExceptT Error (StateT Solver m)
+
+/-- Solver error/state-monad wrapped in `IO`. -/
+abbrev SolverM := SolverT IO
+
+namespace Error
+
+/-- String representation of an error. -/
+protected def toString : Error → String :=
+  toString ∘ repr
+
+/-- Panics on errors, otherwise yields the `ok` result. -/
+def unwrap! [Inhabited α] : Except Error α → α
+| .ok a => a
+| .error e => panic! e.toString
+
+instance : ToString Error :=
+  ⟨Error.toString⟩
+
+end Error
+
+namespace Result
+
+/-- Comparison for structural equality. -/
+protected extern_def beq : Result → Result → Bool
+
+instance : BEq Result := ⟨Result.beq⟩
+
+/-- Hash function for cvc5 sorts. -/
+protected extern_def hash : Result → UInt64
+
+instance : Hashable Result := ⟨Result.hash⟩
+
+/-- True if this result is from a satisfiable `checkSat` or `checkSatAssuming` query. -/
+extern_def isSat : Result → Bool
+
+/-- True if this result is from a unsatisfiable `checkSat` or `checkSatAssuming` query. -/
+extern_def isUnsat : Result → Bool
+
+/-- True if this result is from a `checkSat` or `checkSatAssuming` query and cvc5 was not able to
+determine (un)satisfiability.
+-/
+extern_def isUnknown : Result → Bool
+
+/-- An explanation for an unknown query result.
+
+Note that if the result is (un)sat, this function returns `UnknownExplanation.UNKNOWN_REASON`.
+-/
+extern_def getUnknownExplanation : Result → UnknownExplanation
+with
+  /-- An explanation for an unknown query result, `none` if the result in not unknown. -/
+  getUnknownExplanation? (res : Result) : Option UnknownExplanation :=
+    if ¬ res.isUnknown then none else res.getUnknownExplanation
+
+/-- A string representation of this result. -/
+protected extern_def toString : Result → String
+
+instance : ToString Result := ⟨Result.toString⟩
+
+end Result
+
+section ffi_except_constructors
+
+/-- Only used by FFI to inject values. -/
+@[export except_ok]
+private def mkExceptOk {α : Type} : α → Except Error α :=
+  .ok
+
+/-- Only used by FFI to inject values. -/
+@[export except_ok_bool]
+private def mkExceptOkBool : Bool → Except Error Bool :=
+  .ok
+
+/-- Only used by FFI to inject values. -/
+@[export except_ok_u32]
+private def mkExceptOkU32 : UInt32 → Except Error UInt32 :=
+  .ok
+
+/-- Only used by FFI to inject values. -/
+@[export except_ok_u16]
+private def mkExceptOkU16 : UInt16 → Except Error UInt16 :=
+  .ok
+
+/-- Only used by FFI to inject values. -/
+@[export except_ok_u8]
+private def mkExceptOkU8 : UInt8 → Except Error UInt8 :=
+  .ok
+
+/-- Only used by FFI to inject errors. -/
+@[export except_err]
+private def mkExceptErr {α : Type} : String → Except Error α :=
+  .error ∘ Error.error
+
+end ffi_except_constructors
+
+end cvc5
+
+namespace cvc5.Sort
+
+/-- The null sort. -/
+extern_def null : Unit → cvc5.Sort
+
+instance : Inhabited cvc5.Sort := ⟨null ()⟩
+
+/-- Comparison for structural equality. -/
+protected extern_def beq : cvc5.Sort → cvc5.Sort → Bool
+
+instance : BEq cvc5.Sort := ⟨Sort.beq⟩
+
+/-- Less than comparison. -/
+protected extern_def blt : cvc5.Sort → cvc5.Sort → Bool
+
+/-- Greater than comparison. -/
+protected extern_def bgt : cvc5.Sort → cvc5.Sort → Bool
+
+/-- Less than or equal comparison. -/
+protected extern_def ble : cvc5.Sort → cvc5.Sort → Bool
+
+/-- Greater than or equal comparison. -/
+protected extern_def bge : cvc5.Sort → cvc5.Sort → Bool
+
+/-- Comparison of two sorts. -/
+protected def compare (s1 s2 : cvc5.Sort) : Ordering :=
+  if s1.beq s2 then .eq
+  else if s1.bgt s2 then .gt
+  else .lt
+
+instance : Ord cvc5.Sort := ⟨Sort.compare⟩
+
+instance : LT cvc5.Sort where
+  lt := (Sort.blt · ·)
+
+instance : DecidableLT cvc5.Sort :=
+  fun s1 s2 => if h : s1.blt s2 then .isTrue h else .isFalse h
+
+instance : LE cvc5.Sort where
+  le := (Sort.ble · ·)
+
+instance : DecidableLE cvc5.Sort :=
+  fun s1 s2 => if h : s1.ble s2 then .isTrue h else .isFalse h
+
+/-- Hash function for cvc5 sorts. -/
+protected extern_def hash : cvc5.Sort → UInt64
+
+instance : Hashable cvc5.Sort := ⟨Sort.hash⟩
+
+/-- Get the kind of this sort. -/
+extern_def getKind : cvc5.Sort → SortKind
+
+/-- Determine if this is the null sort (`cvc5.Sort`). -/
+extern_def isNull : cvc5.Sort → Bool
+
+/-- Determine if this is the Boolean sort (SMT-LIB: `Bool`). -/
+extern_def isBoolean : cvc5.Sort → Bool
+
+/-- Determine if this is the Integer sort (SMT-LIB: `Int`). -/
+extern_def isInteger : cvc5.Sort → Bool
+
+/-- Determine if this is the Real sort (SMT-LIB: `Real`). -/
+extern_def isReal : cvc5.Sort → Bool
+
+/-- Determine if this is the String sort (SMT-LIB: `String`). -/
+extern_def isString : cvc5.Sort → Bool
+
+/-- Determine if this is the regular expression sort (SMT-LIB: `RegLan`). -/
+extern_def isRegExp : cvc5.Sort → Bool
+
+/-- Determine if this is the rounding mode sort (SMT-LIB: `RoundingMode`). -/
+extern_def isRoundingMode : cvc5.Sort → Bool
+
+/-- Determine if this is a bit-vector sort (SMT-LIB: `(_ BitVec i)`). -/
+extern_def isBitVector : cvc5.Sort → Bool
+
+/-- Determine if this is a floating-point sort (SMT-LIB: `(_ FloatingPoint eb sb)`). -/
+extern_def isFloatingPoint : cvc5.Sort → Bool
+
+/-- Determine if this is a datatype sort. -/
+extern_def isDatatype : cvc5.Sort → Bool
+
+/-- Determine if this is a datatype constructor sort. -/
+extern_def isDatatypeConstructor : cvc5.Sort → Bool
+
+/-- Determine if this is a datatype selector sort. -/
+extern_def isDatatypeSelector : cvc5.Sort → Bool
+
+/-- Determine if this is a datatype tester sort. -/
+extern_def isDatatypeTester : cvc5.Sort → Bool
+
+/-- Determine if this is a datatype updater sort. -/
+extern_def isDatatypeUpdater : cvc5.Sort → Bool
+
+/-- Determine if this is a function sort. -/
+extern_def isFunction : cvc5.Sort → Bool
+
+/-- Determine if this is a predicate sort.
+
+A predicate sort is a function sort that maps to the Boolean sort. All predicate sorts are also
+function sorts.
+-/
+extern_def isPredicate : cvc5.Sort → Bool
+
+/-- Determine if this is a tuple sort. -/
+extern_def isTuple : cvc5.Sort → Bool
+
+/-- Determine if this is a nullable sort. -/
+extern_def isNullable : cvc5.Sort → Bool
+
+/-- Determine if this is a record sort.
+
+**Warning**: this function is experimental and may change in future versions.
+-/
+extern_def isRecord : cvc5.Sort → Bool
+
+/-- Determine if this is an array sort. -/
+extern_def isArray : cvc5.Sort → Bool
+
+/-- Determine if this is a finite field sort. -/
+extern_def isFiniteField : cvc5.Sort → Bool
+
+/-- Determine if this is a Set sort. -/
+extern_def isSet : cvc5.Sort → Bool
+
+/-- Determine if this is a Bag sort. -/
+extern_def isBag : cvc5.Sort → Bool
+
+/-- Determine if this is a Sequence sort. -/
+extern_def isSequence : cvc5.Sort → Bool
+
+/-- Determine if this is an abstract sort. -/
+extern_def isAbstract : cvc5.Sort → Bool
+
+/-- Determine if this is an uninterpreted sort. -/
+extern_def isUninterpretedSort : cvc5.Sort → Bool
+
+/-- Determine if this is an uninterpreted sort constructor.
+
+An uninterpreted sort constructor has arity `> 0` and can be instantiated to construct uninterpreted
+sorts with given sort parameters.
+-/
+extern_def isUninterpretedSortConstructor : cvc5.Sort → Bool
+
+/-- Determine if this is an instantiated (parametric datatype or uninterpreted sort constructor)
+sort.
+
+An instantiated sort is a sort that has been constructed from instantiating a sort with sort
+arguments --- see also `cvc5.Sort.instantiate`.
+-/
+extern_def isInstantiated : cvc5.Sort → Bool
+
+/-- A string representation of this sort. -/
+protected extern_def toString : cvc5.Sort → String
+
+/-- Determine if this term has a symbol (a name).
+
+For example, free constants and variables have symbols.
+-/
+extern_def!? hasSymbol : cvc5.Sort → Except Error Bool
+
+/-- Get the symbol of this sort.
+
+The symbol of this sort is the string that was provided when consrtucting it *via* one of
+`Solver.mkUninterpretedSort`, `Solver.mkUnresolvedSort`, or
+`Solver.mkUninterpretedSortConstructorSort`.
+-/
+extern_def!? getSymbol : cvc5.Sort → Except Error String
+
+/-- The arity of a function sort. -/
+extern_def!? getFunctionArity : cvc5.Sort → Except Error Nat
+
+/-- The domain sorts of a function sort. -/
+extern_def!? getFunctionDomainSorts : cvc5.Sort → Except Error (Array cvc5.Sort)
+
+/-- The codomain sort of a function sort. -/
+extern_def!? getFunctionCodomainSort : cvc5.Sort → Except Error cvc5.Sort
+
+/-- The array index sort of an array index. -/
+extern_def!? getArrayIndexSort : cvc5.Sort → Except Error cvc5.Sort
+
+/-- The array element sort of an array index. -/
+extern_def!? getArrayElementSort : cvc5.Sort → Except Error cvc5.Sort
+
+/-- The element sort of a set sort. -/
+extern_def!? getSetElementSort : cvc5.Sort → Except Error cvc5.Sort
+
+/-- The element sort of a bag sort. -/
+extern_def!? getBagElementSort : cvc5.Sort → Except Error cvc5.Sort
+
+/-- The element sort of a sequence sort. -/
+extern_def!? getSequenceElementSort : cvc5.Sort → Except Error cvc5.Sort
+
+/-- The sort kind of an abstract sort, which denotes the kind of sorts that this abstract sort
+denotes.
+-/
+extern_def!? getAbstractedKind : cvc5.Sort → Except Error SortKind
+
+/-- The arity of an uninterpreted sort constructor sort. -/
+extern_def!? getUninterpretedSortConstructorArity : cvc5.Sort → Except Error UInt32
+
+/-- The bit-width of the bit-vector sort. -/
+extern_def!? getBitVectorSize : cvc5.Sort → Except Error UInt32
+
+/-- The size of the finite field sort. -/
+extern_def!? getFiniteFieldSize : cvc5.Sort → Except Error Nat
+
+/-- The bit-width of the exponent of the floating-point sort. -/
+extern_def!? getFloatingPointExponentSize : cvc5.Sort → Except Error UInt32
+
+/-- The width of the significand of the floating-point sort. -/
+extern_def!? getFloatingPointSignificandSize : cvc5.Sort → Except Error UInt32
+
+/-- The length of a tuple sort. -/
+extern_def!? getTupleLength : cvc5.Sort → Except Error UInt32
+
+/-- The element sorts of a tuple sort. -/
+extern_def!? getTupleSorts : cvc5.Sort → Except Error (Array cvc5.Sort)
+
+/-- The element sort of a nullable sort. -/
+extern_def!? getNullableElementSort : cvc5.Sort → Except Error cvc5.Sort
+
+/-- Get the associated uninterpreted sort constructor of an instantiated uninterpreted sort. -/
+extern_def!? getUninterpretedSortConstructor : cvc5.Sort → Except Error cvc5.Sort
+
+/-- Instantiate a parameterized datatype sort or uninterpreted sort constructor sort.
+
+Create sort parameters with `TermManager.mkParamSort symbol`.
+
+- `params` The list of sort parameters to instantiate with.
+-/
+extern_def!? instantiate : cvc5.Sort → (params : Array cvc5.Sort) → Except Error cvc5.Sort
+
+/-- Simultaneous substitution of Sorts.
+
+Note that this replacement is applied during a pre-order traversal and only once to the sort. It is not run until fix point. In the case that `sorts` contains duplicates, the replacement earliest in
+the vector takes priority.
+
+**Warning:** This function is experimental and may change in future versions.
+
+- `sorts` The sub-sorts to be substituted within this sort.
+- `replacements` The sort replacing the substituted sub-sorts.
+-/
+extern_def!? substitute
+: cvc5.Sort → (sorts : Array cvc5.Sort) → (replacements : Array cvc5.Sort) → Except Error cvc5.Sort
+
+instance : ToString cvc5.Sort := ⟨Sort.toString⟩
+instance : Repr cvc5.Sort := ⟨fun self _ => self.toString⟩
+
+end cvc5.Sort
+
+namespace cvc5.Op
+
+/-- The null operator. -/
+extern_def null : Unit → Op
+
+instance : Inhabited Op := ⟨null ()⟩
+
+/-- Syntactic equality operator. -/
+protected extern_def beq : Op → Op → Bool
+
+instance : BEq Op := ⟨Op.beq⟩
+
+/-- Get the kind of this operator. -/
+extern_def getKind : Op → Kind
+
+/-- Determine if this operator is nullary. -/
+extern_def isNull : Op → Bool
+
+/-- Determine if this operator is indexed. -/
+extern_def isIndexed : Op → Bool
+
+/-- Get the number of indices of this operator. -/
+extern_def getNumIndices : Op → Nat
+
+/-- Get the index at position `i` of an indexed operator. -/
+protected extern_def get : (op : Op) → Fin op.getNumIndices → Term
+
+/-- Get the string representation of this operator. -/
+protected extern_def toString : Op → String
+
+instance : GetElem Op Nat Term fun op i => i < op.getNumIndices where
+  getElem op i h := op.get ⟨i, h⟩
+
+instance : ToString Op := ⟨Op.toString⟩
+
+end Op
+
+namespace Term
+
+/-- The null term. -/
+extern_def null : Unit → Term
+
+instance : Inhabited Term := ⟨null ()⟩
+
+/-- Syntactic equality operator. -/
+protected extern_def beq : Term → Term → Bool
+
+instance : BEq Term := ⟨Term.beq⟩
+
+protected extern_def hash : Term → UInt64
+
+instance : Hashable Term := ⟨Term.hash⟩
+
+/-- Determine if this term is nullary. -/
+extern_def isNull : Term → Bool
+
+/-- Get the kind of this term. -/
+extern_def getKind : Term → Kind
+
+/-- Get the sort of this term. -/
+extern_def getSort : Term → cvc5.Sort
+
+/-- Determine if this term has an operator. -/
+extern_def hasOp : Term → Bool
+
+/-- Determine if this term has a symbol (a name).
+
+For example, free constants and variables have symbols.
+-/
+extern_def hasSymbol : Term → Bool
+
+/-- Get the id of this term. -/
+extern_def getId : Term → Nat
+
+/-- Get the number of children of this term. -/
+extern_def getNumChildren : Term → Nat
+
+/-- Is this term a skolem? -/
+extern_def isSkolem : Term → Bool
+
+/-- Get the child term of this term at a given index. -/
+protected extern_def get : (t : Term) → Fin t.getNumChildren → Term
+
+/-- Get the operator of a term with an operator.
+
+Requires that this term has an operator (see `hasOp`).
+-/
+extern_def!? getOp : Term → Except Error Op
+
+/-- Get the value of a Boolean term as a native Boolean value.
+
+Requires `term` to have sort Bool.
+-/
+extern_def!? getBooleanValue : Term → Except Error Bool
+
+/-- Get the string representation of a bit-vector value.
+
+Requires `term` to have a bit-vector sort.
+
+- `base`: `2` for binary, `10` for decimal, and `16` for hexadecimal.
+-/
+extern_def!? getBitVectorValue : Term → UInt32 → Except Error String
+
+/-- Get the native integral value of an integral value. -/
+extern_def!? getIntegerValue : Term → Except Error Int
+
+/-- Get the native rational value of a real, rational-compatible value. -/
+extern_def!? getRationalValue : Term → Except Error Std.Internal.Rat
+
+/-- Get the symbol of this term.
+
+Requires that this term has a symbol (see `hasSymbol`).
+
+The symbol of the term is the string that was provided when constructing it *via*
+`TermManager.mkConst` or `TermManager.mkVar`.
+-/
+extern_def!? getSymbol : Term → Except Error String
+
+/-- Get skolem identifier of this term.
+
+Requires `isSkolem`.
+-/
+extern_def!? getSkolemId : Term → Except Error SkolemId
+
+/-- Get the skolem indices of this term.
+
+Requires `isSkolem`.
+
+Returns the skolem indices of this term. This is a list of terms that the skolem function is indexed
+by. For example, the array diff skolem `SkolemId.ARRAY_DEQ_DIFF` is indexed by two arrays.
+-/
+extern_def!? getSkolemIndices : Term → Except Error (Array Term)
+
+instance : GetElem Term Nat Term fun t i => i < t.getNumChildren where
+  getElem t i h := t.get ⟨i, h⟩
+
+protected def forIn {β : Type u} [Monad m] (t : Term) (b : β) (f : Term → β → m (ForInStep β)) : m β :=
+  let rec loop (i : Nat) (h : i ≤ t.getNumChildren) (b : β) : m β := do
+    match i, h with
+    | 0,   _ => pure b
+    | i+1, h =>
+      have h' : i < t.getNumChildren := Nat.lt_of_lt_of_le (Nat.lt_succ_self i) h
+      have : t.getNumChildren - 1 < t.getNumChildren := Nat.sub_lt (Nat.zero_lt_of_lt h') (by decide)
+      have : t.getNumChildren - 1 - i < t.getNumChildren := Nat.lt_of_le_of_lt (Nat.sub_le (t.getNumChildren - 1) i) this
+      match (← f t[t.getNumChildren - 1 - i] b) with
+      | ForInStep.done b  => pure b
+      | ForInStep.yield b => loop i (Nat.le_of_lt h') b
+  loop t.getNumChildren (Nat.le_refl _) b
+
+instance : ForIn m Term Term where
+  forIn := Term.forIn
+
+/-- Get the children of a term. -/
+def getChildren (t : Term) : Array Term := Id.run do
+  let mut cts := #[]
+  for ct in t do
+    cts := cts.push ct
+  cts
+
+/-- Boolean negation. -/
+protected extern_def!? not : (t : Term) → Except Error Term
+
+/-- Boolean and. -/
+protected extern_def!? and : (lft rgt : Term) → Except Error Term
+
+/-- Boolean or. -/
+protected extern_def!? or : (lft rgt : Term) → Except Error Term
+
+/-- Boolean exclusive or. -/
+protected extern_def!? xor : (lft rgt : Term) → Except Error Term
+
+/-- Equality. -/
+protected extern_def!? eq : (lft rgt : Term) → Except Error Term
+
+/-- Boolean implication. -/
+protected extern_def!? imp : (lft rgt : Term) → Except Error Term
+
+/-- If-then-else.
+
+- `cnd`: condition, must be a Boolean term;
+- `thn`: then-branch of some sort `S`;
+- `els`: else-branch of *the same* sort `S`.
+-/
+protected extern_def!? ite : (cnd thn els : Term) → Except Error Term
+
+/-- A string representation of this term. -/
+protected extern_def toString : Term → String
+
+instance : ToString Term := ⟨Term.toString⟩
+
+end Term
+
+namespace Proof
+
+/-- The null proof. -/
+extern_def null : Unit → Proof
+
+instance : Inhabited Proof := ⟨null ()⟩
+
+/-- Get the proof rule used by the root step of the root. -/
+extern_def getRule : Proof → ProofRule
+
+/-- Get the proof rewrite rule used by the root step of the proof.
+
+Requires that `getRule` does not return `ProofRule.DSL_REWRITE` or `ProofRule.REWRITE`.
+-/
+extern_def!? getRewriteRule : Proof → Except Error ProofRewriteRule
+
+/-- The conclusion of the root step of the proof. -/
+extern_def getResult : Proof → Term
+
+/-- The premises of the root step of the proof. -/
+extern_def getChildren : Proof → Array Proof
+
+/-- The arguments of the root step of the proof as a vector of terms.
+
+Some of those terms might be strings.
+-/
+extern_def getArguments : Proof → Array Term
+
+/-- Operator overloading for referential equality of two proofs. -/
+protected extern_def beq : Proof → Proof → Bool
+
+instance : BEq Proof := ⟨Proof.beq⟩
+
+/-- Hash function for proofs. -/
+protected extern_def hash : Proof → UInt64
+
+instance : Hashable Proof := ⟨Proof.hash⟩
+
+end Proof
+
+namespace TermManager
+
+/-- Constructor. -/
+extern_def new : BaseIO TermManager
+
+/-- Get the Boolean sort. -/
+extern_def getBooleanSort : TermManager → cvc5.Sort
+
+/-- Get the Integer sort. -/
+extern_def getIntegerSort : TermManager → cvc5.Sort
+
+/-- Get the Real sort. -/
+extern_def getRealSort : TermManager → cvc5.Sort
+
+/-- Get the regular expression sort. -/
+extern_def getRegExpSort : TermManager → cvc5.Sort
+
+/-- Get the rounding mode sort. -/
+extern_def getRoundingModeSort : TermManager → cvc5.Sort
+
+/-- Get the string sort. -/
+extern_def getStringSort : TermManager → cvc5.Sort
+
+/-- Create an array sort.
+
+- `indexSort` The array index sort.
+- `elemSort` The array element sort.
+-/
+extern_def!? mkArraySort : TermManager → (indexSort elemSort : cvc5.Sort) → Except Error cvc5.Sort
+
+/-- Create a bit-vector sort.
+
+- `size` The bit-width of the bit-vector sort.
+-/
+extern_def!? mkBitVectorSort : TermManager → (size : UInt32) → Except Error cvc5.Sort
+
+/-- Create a floating-point sort.
+
+- `exp` The bit-width of the exponent of the floating-point sort.
+- `sig` The bit-width of the significand of the floating-point sort.
+-/
+extern_def!? mkFloatingPointSort : TermManager → (exp sig : UInt32) → Except Error cvc5.Sort
+
+/-- Create a finite-field sort from a given string of base n.
+
+- `size` The modulus of the field. Must be a prime.
+-/
+private extern_def mkFiniteFieldSortFromString : TermManager → (size : String) → (base : UInt32 := 10) → Except Error cvc5.Sort
+
+@[inherit_doc mkFiniteFieldSortFromString]
+abbrev mkFiniteFieldSort (tm : TermManager) : (size : Nat) → Except Error cvc5.Sort :=
+  (tm.mkFiniteFieldSortFromString · 10) ∘ toString
+@[inherit_doc mkFiniteFieldSortFromString]
+abbrev mkFiniteFieldSort! (tm : TermManager) : (size : Nat) → cvc5.Sort :=
+  Error.unwrap! ∘ (tm.mkFiniteFieldSortFromString · 10) ∘ toString
+@[inherit_doc mkFiniteFieldSortFromString]
+abbrev mkFiniteFieldSort? (tm : TermManager) : (size : Nat) → Option cvc5.Sort :=
+  Except.toOption ∘ (tm.mkFiniteFieldSortFromString · 10) ∘ toString
+
+/-- Create function sort.
+
+- `sorts` The sort of the function arguments.
+- `codomain` The sort of the function return value.
+-/
+extern_def!? mkFunctionSort
+: TermManager → (sorts : Array cvc5.Sort) → (codomain : cvc5.Sort) → Except Error cvc5.Sort
+
+/-- Create a predicate sort.
+
+This is equivalent to calling `mkFunctionSort` with Boolean sort as the codomain.
+
+- `sorts` The list of sorts of the predicate.
+-/
+extern_def!? mkPredicateSort : TermManager → (sorts : Array cvc5.Sort) → Except Error cvc5.Sort
+
+/-- Create a tuple sort.
+
+- `sorts` The sorts of the elements of the tuple.
+-/
+extern_def!? mkTupleSort : TermManager → (sorts : Array cvc5.Sort) → Except Error cvc5.Sort
+
+/-- Create an uninterpreted sort constructor sort.
+
+An uninterpreted sort constructor is an uninterpreted sort with arity > 0.
+
+- `arity` The arity of the sort (must be > 0).
+- `symbol` The symbol of the sort.
+-/
+extern_def!? mkUninterpretedSortConstructorSort
+: TermManager → (arity : Nat) → (symbol : String) → Except Error cvc5.Sort
+
+/-- Create a set parameter.
+
+- `elemSort` The sort of the set elements.
+-/
+extern_def!? mkSetSort : TermManager → (sort : cvc5.Sort) → Except Error cvc5.Sort
+
+/-- Create a set parameter.
+
+- `elemSort` The sort of the set elements.
+-/
+extern_def!? mkBagSort : TermManager → (sort : cvc5.Sort) → Except Error cvc5.Sort
+
+/-- Create a set parameter.
+
+- `elemSort` The sort of the set elements.
+-/
+extern_def!? mkSequenceSort : TermManager → (sort : cvc5.Sort) → Except Error cvc5.Sort
+
+/-- Create an abstract sort. An abstract sort represents a sort for a given kind whose parameters
+and arguments are unspecified.
+
+The kind `k` must be the kind of a sort that can be abstracted, *i.e.* a sort that has indices or
+arguments sorts. For example, `SortKind.ARRAY_SORT` and `SortKind.BITVECTOR_SORT` can be passed as
+the kind `k` to this function, while `SortKind.INTEGER_SORT` and `SortKind.STRING_SORT` cannot.
+
+**NB:** Providing the kind `SortKind.ABSTRACT_SORT` as an argument to this function returns the
+(fully) unspecified sort, denoted `?`.
+
+**NB:** Providing a kind `k` that has no indices and a fixed arity of argument sorts will return the
+sort of kind `k` whose arguments are the unspecified sort. For example, `mkAbstractSort
+SortKind.ARRAY_SORT` will return the sort `(ARRAY_SORT ? ?)` instead of the abstract sort whose
+abstract kind is `SortKind.ARRAY_SORT`.
+-/
+extern_def!? mkAbstractSort : TermManager → (k : SortKind) → Except Error cvc5.Sort
+
+/-- Create an uninterpreted sort.
+
+- `symbol` The name of the sort.
+-/
+extern_def mkUninterpretedSort : TermManager → (symbol : String) → cvc5.Sort
+
+/-- Create a nullable sort.
+
+- `sort` The sort of the element of the nullable.
+-/
+extern_def!? mkNullableSort : TermManager → (sort : cvc5.Sort) → Except Error cvc5.Sort
+
+/-- Create a sort parameter.
+
+- `symbol` The name of the sort.
+
+**Warning**: This function is experimental and may change in future versions.
+-/
+extern_def mkParamSort : TermManager → (symbol : String) → cvc5.Sort
+
+/-- Create a Boolean constant.
+
+- `b`: The Boolean constant.
+-/
+extern_def mkBoolean : TermManager → (b : Bool) → Term
+
+/-- Create an integer-value term.
+
+- `s`: the string representation of the constant, may represent an integer such as (`"123"`).
+-/
+private extern_def mkIntegerFromString : TermManager → (s : String) → Except Error Term
+with
+  /-- Create an integer-value term. -/
+  mkInteger (tm : TermManager) : Int → Term :=
+    Error.unwrap! ∘ tm.mkIntegerFromString ∘ toString
+
+/-- Create a real-value term.
+
+- `s`: the string representation of the constant, may represent an integer (`"123"`) or a real
+  constant (`"12.34"`, `"12/34"`).
+-/
+private extern_def mkRealFromString : TermManager → (s : String) → Except Error Term
+with
+  /-- Create a real-value term from a `Std.Internal.Rat`. -/
+  mkRealOfRat (tm : TermManager) (rat : Std.Internal.Rat) : Term :=
+    tm.mkRealFromString s!"{rat.num}/{rat.den}" |> Error.unwrap!
+  /-- Create a real-value term from numerator/denominator `Int`-s. -/
+  mkReal (tm : TermManager)
+    (num : Int) (den : Int := 1) (den_ne_0 : den ≠ 0 := by simp <;> omega)
+  : Term :=
+    let (num, den) :=
+      match h : den with
+      | .ofNat 0 => by contradiction
+      | .ofNat den => (num, den)
+      | .negSucc denMinus1 => (-num, denMinus1.succ)
+    tm.mkRealOfRat <| Std.Internal.mkRat num den
+
+/-- Create operator of Kind:
+
+- `Kind.BITVECTOR_EXTRACT`
+- `Kind.BITVECTOR_REPEAT`
+- `Kind.BITVECTOR_ROTATE_LEFT`
+- `Kind.BITVECTOR_ROTATE_RIGHT`
+- `Kind.BITVECTOR_SIGN_EXTEND`
+- `Kind.BITVECTOR_ZERO_EXTEND`
+- `Kind.DIVISIBLE`
+- `Kind.FLOATINGPOINT_TO_FP_FROM_FP`
+- `Kind.FLOATINGPOINT_TO_FP_FROM_IEEE_BV`
+- `Kind.FLOATINGPOINT_TO_FP_FROM_REAL`
+- `Kind.FLOATINGPOINT_TO_FP_FROM_SBV`
+- `Kind.FLOATINGPOINT_TO_FP_FROM_UBV`
+- `Kind.FLOATINGPOINT_TO_SBV`
+- `Kind.FLOATINGPOINT_TO_UBV`
+- `Kind.INT_TO_BITVECTOR`
+- `Kind.TUPLE_PROJECT`
+
+See `cvc5.Kind` for a description of the parameters.
+
+- `kind` The kind of the operator.
+- `args` The arguments (indices) of the operator.
+
+If `args` is empty, the `Op` simply wraps the `cvc5.Kind`. The `Kind` can be used in
+`Solver.mkTerm` directly without creating an `Op` first.
+-/
+extern_def!? mkOpOfIndices : TermManager → (kind : Kind) → (args : Array Nat := #[]) → Except Error Op
+
+@[inherit_doc mkOpOfIndices]
+abbrev mkOp := @mkOpOfIndices
+@[inherit_doc mkOpOfIndices!]
+abbrev mkOp! := @mkOpOfIndices!
+@[inherit_doc mkOpOfIndices?]
+abbrev mkOp? := @mkOpOfIndices?
+
+/-- Create operator of kind:
+
+- `Kind.DIVISIBLE` (to support arbitrary precision integers)
+
+See `cvc5.Kind` for a description of the parameters.
+
+- `kind` The kind of the operator.
+- `arg` The string argument to this operator.
+-/
+extern_def!? mkOpOfString : TermManager → (kind : Kind) → (arg : String) → Except Error Op
+
+/-- Create n-ary term of given kind.
+
+- `kind` The kind of the term.
+- `children` The children of the term.
+-/
+extern_def!? mkTerm : TermManager → (kind : Kind) → (children : Array Term := #[]) → Except Error Term
+
+/-- Create n-ary term of given kind from a given operator.
+
+Create operators with `mkOp`.
+
+- `op` The operator.
+- `children` The children of the term.
+-/
+extern_def!? mkTermOfOp : TermManager → (op : Op) → (children : Array Term := #[]) → Except Error Term
+
+/-- **THIS FUNCTION MUST NOT BE EXPOSED.**
+
+**It produces a different (fresh) term every time it's called which is really bad for purity.**
+
+Create a free constant.
+
+Note that the returned term is always fresh, even if the same arguments were provided on a
+previous call to `mkConst`.
+
+- `sort` The sort of the constant.
+- `symbol` The name of the constant (optional).
+-/
+private
+def mkConst (_ : TermManager) (_ : cvc5.Sort) (_ : String := "") : Term :=
+  panic! "illegal call to `cvc5.TermManager.mkConst"
+
+end TermManager
+
+namespace Solver
+
+variable [Monad m]
+
+/-- Only used by FFI to wrap *success* results. -/
+@[export solver_val]
+private def val (a : α) : SolverT m α := pure a
+
+/-- Only used by FFI to wrap errors. -/
+@[export solver_err]
+private def err (e : Error) : SolverT m α := throw e
+
+/-- Only used by FFI to wrap cvc5 errors. -/
+@[export solver_errOfString]
+private def errorOfString (msg : String) : SolverT m α := throw (.error msg)
+
+/-- Constructor.
+
+Constructs solver instance from a given term manager instance.
+
+- `tm`: The associated term manager.
+-/
+private extern_def new : TermManager → Solver
+
+/-- Get a string representation of the version of this solver. -/
+extern_def getVersion : SolverT m String
+
+/-- Set option.
+
+- `option`: The option name.
+- `value`: The option value.
+-/
+extern_def setOption (option value : String) : SolverT m Unit
+
+/-- Remove all assertions. -/
+extern_def resetAssertions : SolverT m Unit
+
+/-- Set logic.
+
+- `logic`: The logic to set.
+-/
+extern_def setLogic : (logic : String) → SolverT m Unit
+
+/-- Simplify a term or formula based on rewriting and (optionally) applying substitutions for
+solved variables.
+
+If `applySubs` is true, then for example, if `(= x 0)` was asserted to this solver, this function
+may replace occurrences of `x` with `0`.
+
+- `t` The term to simplify.
+- `applySubs` True to apply substitutions for solved variables.
+-/
+extern_def simplify : (term : Term) → (applySubs : Bool := false) → SolverT m Term
+
+/--
+Declare n-ary function symbol.
+
+SMT-LIB:
+
+\verbatim embed:rst:leading-asterisk
+ .. code:: smtlib
+
+     (declare-fun <symbol> ( <sort>* ) <sort>)
+ \endverbatim
+
+- `symbol`: The name of the function.
+- `sorts`: The sorts of the parameters to this function.
+- `sort`: The sort of the return value of this function.
+- `fresh`: If true, then this method always returns a new Term. Otherwise, this method will always
+  return the same Term for each call with the given sorts and symbol where fresh is false.
+-/
+extern_def declareFun (symbol : String) (sorts : Array cvc5.Sort) (sort : cvc5.Sort) (fresh := true) : SolverT m Term
+
+/-- Assert a formula.
+
+- `term`: The formula to assert.
+-/
+extern_def assertFormula : Term → SolverT m Unit
+
+/-- Check satisfiability. -/
+extern_def checkSat : SolverT m Result
+
+/-- Check satisfiability assuming the given formulas.
+
+- `assumptions`: The formulas to assume.
+-/
+extern_def checkSatAssuming : (assumptions : Array Term) → SolverT m Result
+
+/-- Get a proof associated with the most recent call to `checkSat`.
+
+Requires to enable option `produce-proofs`.
+-/
+extern_def getProof : SolverT m (Array Proof)
+
+/--
+Get the values of the given term in the current model.
+
+SMT-LIB:
+
+\verbatim embed:rst:leading-asterisk
+.. code:: smtlib
+
+    (get-value ( <term>* ))
+\endverbatim
+
+- `terms`: The term for which the value is queried.
+-/
+extern_def getValue (term : Term) : SolverT m Term
+
+/--
+Get the values of the given terms in the current model.
+
+SMT-LIB:
+
+\verbatim embed:rst:leading-asterisk
+.. code:: smtlib
+
+    (get-value ( <term>* ))
+\endverbatim
+
+- `terms`: The terms for which the values are queried.
+-/
+extern_def getValues (terms : Array Term) : SolverT m (Array Term)
+
+/-- Prints a proof as a string in a selected proof format mode.
+
+Other aspects of printing are taken from the solver options.
+
+- `proof`: A proof, usually obtained from `getProof`.
+-/
+extern_def proofToString : Proof → SolverT m String
+
+/-- Parse a string containing SMT-LIB commands.
+
+Commands that produce a result such as `(check-sat)`, `(get-model)`, ... are executed but the
+results are ignored.
+-/
+extern_def parseCommands : String → SolverT m Unit
+
+/-- Run a `query` given a term manager `tm`. -/
+def run (tm : TermManager) (query : SolverT m α) : m (Except Error α) :=
+  return match ← ExceptT.run query (new tm) with
+  | (.ok x, _) => .ok x
+  | (.error e, _) => .error e
+
+/-- Run a `query` given a term manager `tm`. -/
+def run! [Inhabited α] (tm : TermManager) (query : SolverT m α) : m α := do
+  match ← ExceptT.run query (new tm) with
+  | (.ok x, _) => return x
+  | (.error e, _) => do
+    panic! s!"{e}"
+
+end Solver
+
+end cvc5
