cvc5/NuInit.lean
@@ -1,0 +1,378 @@
+/-
+Copyright (c) 2023-2024 by the authors listed in the file AUTHORS and their
+institutional affiliations. All rights reserved.
+Released under Apache 2.0 license as described in the file LICENSE.
+Authors: Abdalrhman Mohamed, Adrien Champion
+-/
+
+import Lean.Elab.Command
+
+namespace Cvc5
+
+/-! ## DSL for definition  DRY -/
+section defsMacro
+
+open Lean
+open Elab
+open Command (CommandElab CommandElabM)
+
+declare_syntax_cat externKw'
+
+declare_syntax_cat defsItem'
+declare_syntax_cat defsItemHead'
+declare_syntax_cat defsItemTail!?'
+declare_syntax_cat defsItemTail'
+
+declare_syntax_cat defsMod
+
+/-- Arity of an expression.
+
+Stolen from [batteries].
+
+[batteries]: https://leanprover-community.github.io/mathlib4_docs/Batteries/Lean/Expr.html#Lean.Expr.forallArity
+-/
+def forallArity : Expr → Nat
+  | .mdata _ b => forallArity b
+  | .forallE _ _ body _ => forallArity body
+  | _ => 0
+
+syntax "?" : defsMod
+syntax "!" : defsMod
+syntax "!?" : defsMod
+syntax "?!" : defsMod
+
+scoped syntax (name := defsItemStxHead')
+  declModifiers
+  ("@[" "force" str "]")?
+  "def " defsMod ? ident
+: defsItemHead'
+
+scoped syntax (name := defsItemStxTail!?')
+  withPosition(ppLine "with!? "
+    group(
+      colGt
+      docComment ?
+      ident
+    )*
+  )
+: defsItemTail!?'
+
+scoped syntax (name := defsItemStxTail')
+  withPosition(ppLine "with "
+    group(
+      colGt
+      docComment ?
+      declId optDeclSig ":= " withPosition(group(colGe term))
+    )*
+  )
+: defsItemTail'
+
+scoped syntax (name := defsItemStx')
+  defsItemHead'
+  declSig
+  (defsItemTail!?')?
+  (defsItemTail')?
+: defsItem'
+
+unsafe def elabDefsItem
+  (pref : String) (forceMods : Option (TSyntax `defsMod))
+: CommandElab
+| `(defsItem'|
+    $mods:declModifiers
+    $[ @[ force $forcedName ] ]?
+    def $ident:ident $identSig:declSig
+    $[ with!? $[
+        $[$autoDoc]?
+        $autoId
+    ]* ]?
+    $[ with $[
+        $[$subDoc]?
+        $subId $subSig := $subDef
+    ]* ]?
+) => do
+  if let some defMods := forceMods then
+    let stx ← `(defsItem'|
+$mods:declModifiers
+$[ @[ force $forcedName ] ]?
+def $defMods $ident:ident $identSig:declSig
+$[ with!? $[
+    $[$autoDoc]?
+    $autoId
+]* ]?
+$[ with $[
+    $[$subDoc]?
+    $subId $subSig := $subDef
+]* ]?
+    )
+    return ← elabDefsItem pref none stx
+
+  let externName :=
+    let id :=
+      if let some forcedName := forcedName then
+        forcedName.getString
+      else
+        ident.getId.toString
+    pref ++ "_" ++ id |> Syntax.mkStrLit
+  -- println! "pref = {pref}"
+  let mods ←
+    match mods with
+    | `(Parser.Command.declModifiersT|
+      $[$doc:docComment]? $[@[ $[ $attrs ],* ]]? $[$vis]? $[$isNc]? $[$isUnsafe]? $[$opt]?
+    ) => do
+      let ext ← `(Parser.Term.attrInstance| extern $externName:str)
+      let attrs := attrs.getD #[] |>.push ext
+      `(Parser.Command.declModifiersT|
+        $[$doc:docComment]? @[ $[$attrs],* ] $[$vis]? $[$isNc]? $[$isUnsafe]? $[$opt]?
+      )
+    | _ => throwUnsupportedSyntax
+  let mainDef ←`(
+    set_option linter.unusedVariables false in
+    $(⟨mods⟩):declModifiers
+    opaque $ident:declId $identSig
+  )
+  Command.elabCommand mainDef
+
+  let fullName :=
+    Lean.Name.mkSimple ident.getId.toString
+    |> (← Elab.liftMacroM Macro.getCurrNamespace).append
+  let fullIdent := Lean.mkIdent fullName
+
+  let define doc? id sig? (body : Syntax.Term) : CommandElabM _ := do
+    if let some doc := doc? then
+      `(command|
+        $doc:docComment
+        def $id:declId $sig?:optDeclSig := $body
+      )
+    else
+      `(command|
+        @[inherit_doc $fullIdent]
+        def $id:declId $sig?:optDeclSig := $body
+      )
+
+  if let (some autoDoc?, some autoId) := (autoDoc, autoId) then
+    let env ← getEnv
+    let arity ←
+      if let some (.opaqueInfo i) := env.find? fullName then
+        pure i.type.getForallArity
+      else
+        throwError s!"failed to retrieve arity of (opaque) function `{ident}`"
+
+    let mut args := #[ Lean.Name.mkSimple "ω" |> Lean.mkIdent ]
+    for i in [0:arity.pred] do
+      let arg := Lean.Name.mkSimple s!"v{i}" |> Lean.mkIdent
+      args := args.push arg
+    let funCall : TSyntax `term ← `(term| ( @ $fullIdent $[ $args ]* ))
+
+    for (autoDoc?, autoId) in autoDoc?.zip autoId do
+      let id : String := autoId.getId.toString
+      let body ←
+        if id.endsWith "!" then
+          let unwrapName := Lean.Name.mkStr3 "Cvc5" "Error" "unwrap!" |> Lean.mkIdent
+          `(fun $[$args]* => $funCall |> $unwrapName)
+        else if id.endsWith "?" then
+          `(fun $[$args]* => $funCall |> Except.toOption)
+        else
+          throwError s!"unexpected auto function name `{id}`: expected `<ident>!` or `<ident>?`"
+      let cmd ← define autoDoc? autoId (← `(optDeclSig|)) body
+      Command.elabCommand cmd
+
+  if let
+    (some subDoc?, some subId, some subSig, some subDef)
+    := (subDoc, subId, subSig, subDef)
+  then
+    let all := subDoc?.zip subId |>.zip subSig |>.zip subDef
+    for (((subDoc?, subId), subSig), subDef) in all do
+      Command.elabCommand
+        (← define subDoc? subId subSig subDef)
+| `(defsItem'|
+    $mods:declModifiers
+    $[ @[ force $forcedName ] ]?
+    def $defsMod $ident:ident $identSig:declSig
+    $[ with $[
+        $[$subDoc]?
+        $subId $subSig := $subDef
+    ]* ]?
+) => do
+  let name := ident.getId
+  let identOpt _ := name.appendAfter "?" |> Lean.mkIdent
+  let identPanic _ := name.appendAfter "!" |> Lean.mkIdent
+  let auto : Array Ident ←
+    match defsMod with
+    | `(defsMod| ?) => pure #[identOpt ()]
+    | `(defsMod| !) => pure #[identPanic ()]
+    | `(defsMod| ?!)
+    | `(defsMod| !?) => pure #[identOpt (), identPanic ()]
+    | _ => throwUnsupportedSyntax
+  let stx ← `(defsItemStx'|
+    $mods:declModifiers
+    $[ @[ force $forcedName ] ]?
+    def $ident:ident $identSig:declSig
+    with!? $[ $auto:ident ]*
+    $[ with $[
+        $[ $subDoc:docComment ]?
+        $subId:declId $subSig:optDeclSig := $subDef:term
+    ]* ]?
+  )
+  elabDefsItem pref none stx
+| _ => throwUnsupportedSyntax
+
+/-- Defines similar functions realized by `extern`.
+
+```
+extern! in "prefix"
+  /-- Create a Boolean constant.
+
+  - `b`: The Boolean constant.
+
+  Will create an opaque definition with `[@extern extStr]` where
+  `extStr = "prefix" ++ "_" ++ "myFunction"`.
+  -/
+  def myFunction : Term → Except Error Op
+  with!?
+    endsWithBang!
+    endWithQuestion?
+  with
+    myOtherFunction : Term → Op :=
+      Error.unwrap! ∘ myFunction
+    /-- Optional function docstring: if none, inherit from the main function. -/
+    yetAnotherFunction : Term → Option Op :=
+      Except.toOption ∘ myFunction
+```
+
+- `in "prefix"` is optional; if none, then the prefix will be the (last component of the) name of
+  the current namespace with the first letter lowercased. Fails if the current namespace has no
+  components.
+
+- `with ...`: takes a sequence of identifiers, each generate a function that
+  - unwraps the result if `!`-ended, which generates code similar to `myOtherFunction` above;
+  - turns a result into an option if `?`-ended, which generates code similar to `yetAnotherFunction`
+    above;
+  - fails otherwise.
+
+  The `with ...` syntax is currently only compatible with external functions that produce `Except
+  Error α` values.
+
+- Supports `declModifiers` on the main (`def`) function `myFunction` such as `private`.
+- Accepts a list of external (`def`) functions, each with its `with` clauses.
+
+This macro can generate optional (`?`) and panic (`!`) wrappers even more automatically.
+
+```
+extern! "prefix"
+  /-- Create a Boolean constant.
+
+  - `b`: The Boolean constant.
+
+  Will create an opaque definition with `[@extern extStr]` where
+  `extStr = "prefix" ++ "_" ++ "myFunction"`.
+  -/
+  def !? myFunction : Term → Except Error Op
+  with
+    myOtherFunction : Term → Op :=
+      myFunction!
+    /-- Optional function docstring: if none, inherit from the main function. -/
+    yetAnotherFunction : Term → Option Op :=
+      myFunction?
+```
+
+Notice the `!?` between `def` and `myFunction`. This generates `myFunction!` and `myFunction?` which
+respectively panic-unwrap errors and turn the `Except` into an `Option`. In other words, it is the
+same as (and internally turned into) a `with!? myFunction! myFunction?` clause using the first
+syntax above.
+
+Besides `!?`, the following are also supported:
+- `?!`: same behavior as `!?`;
+- `!`: only generate the panic unwrapper;
+- `?`: only generate the `Option` unwrapper.
+-/
+scoped syntax (name := multidefs)
+  withPosition("external! " ("in " str)? ppLine group(colGt defsItem')+)
+: command
+
+@[inherit_doc multidefs, command_elab multidefs]
+unsafe def multidefsImpl : CommandElab
+| `(command|
+  external! $[in $pref:str]? $[$defsItems']*
+) => do
+  let ns ← getCurrNamespace
+  let pref ←
+    if let some pref := pref then
+      pure pref.getString
+    else
+      -- println! "componentsRev for {ns.toString}"
+      -- for c in ns.componentsRev do
+      --   println! "- {c.toString}"
+      if let super::_ := ns.componentsRev then
+        let mut super := super.toString
+        if 0 < super.length then
+          super := super.get 0 |>.toLower |> super.set 0
+        -- println! "-> `{super}`"
+        pure <| if super = "srt" then "sort" else super
+      else
+        throwError "failed to retrieve current workspace, please provide an explicit prefix"
+  for defsItem' in defsItems' do
+    elabDefsItem pref none defsItem'
+| _ => throwUnsupportedSyntax
+
+scoped syntax (name := externkw)
+  ("extern_def " <|> "extern_def! " <|> "extern_def? " <|> "extern_def!? " <|> "extern_def?! ")
+: externKw'
+
+/-- Defines an external, opaque function with optional helpers.
+
+```
+/-- Some documentation. -/
+extern_def!? in "prefix" myFunction : Term → Except Error Op
+```
+
+Generates an opaque definition
+
+```
+/-- Some documentation. -/
+@[extern "prefix_myFunction"]
+def myFunction : Term → Except Error Op
+```
+
+- `in "prefix"` is optional, uses the current namespace with first letter lowercased if none.
+
+- `extern_def!?` also defines `myFunction! : Term → Op` and `myFunction? : Term → Option Op` in
+  terms of `myFunction`.
+
+  Other variants exist:
+  - `extern_def?!`: same as `extern_def!?`;
+  - `extern_def?`: only defines `myFunction?`;
+  - `extern_def!`: only defines `myFunction!`;
+  - `extern_def`: defines nothing besides `myFunction`.
+-/
+scoped syntax (name := externdef)
+  declModifiers
+  withPosition(
+    externKw'
+    ("in " str)?
+    ident declSig (defsItemTail')?
+  )
+: command
+
+@[inherit_doc externdef, command_elab externdef]
+unsafe def externdefImpl : CommandElab
+| `(command|
+  $mods:declModifiers
+  $externKw' $[in $path:str]? $ident $sig $[$tail]?
+) => do
+  let defMod ←
+    match externKw' with
+    | `(externKw'| extern_def) => pure none
+    | `(externKw'| extern_def!) => `(defsMod| !)
+    | `(externKw'| extern_def?) => `(defsMod| ?)
+    | `(externKw'| extern_def!?) => `(defsMod| !?)
+    | `(externKw'| extern_def?!) => `(defsMod| ?!)
+    | _ => throwUnsupportedSyntax
+  let stx ← `(
+    external! $[in $path]?
+      $mods:declModifiers
+      def $[$defMod]? $ident $sig $[$tail:defsItemTail']?
+  )
+  Command.elabCommand stx
+| _ => throwUnsupportedSyntax
+
+end defsMacro
