cvcTests/Test.lean
@@ -1,0 +1,22 @@
+import cvc5
+
+
+
+namespace Cvc5.Test
+
+/-- info: bool = `Bool` -/
+#guard_msgs in #eval Env.runIO do
+  let bool ← Env.getBooleanSort
+  println! "bool = `{bool}`"
+
+/-- error: [error] not a function sort: Bool -/
+#guard_msgs in #eval Env.runIO do
+  let bool ← Env.getBooleanSort
+  let _sorts ← bool.getFunctionDomainSorts
+
+/-- info: x = `x` -/
+#guard_msgs in #eval Env.runIO do
+  let bool ← Env.getBooleanSort
+  let solver ← Solver.new
+  let x ← solver.declareFun "x" #[] bool
+  println! "x = `{x}`"
